WIP refactor

theories/Assert.v
@@ -1,8 +1,8 @@
 From CoindSemWhile Require Import SsrExport Trace Language.
 
-Add Relation trace bisim 
+Add Relation trace bisim
 reflexivity proved by bisim_reflexive
-symmetry proved by bisim_symmetric 
+symmetry proved by bisim_symmetric
 transitivity proved by bisim_transitive
 as bisim_rel.
 
@@ -11,7 +11,7 @@ Unset Strict Implicit.
 Import Prenex Implicits.
 
 Definition setoid (p: trace -> Prop) :=
-forall tr0, p tr0 -> forall tr1, bisim tr0 tr1 -> p tr1.  
+forall tr0, p tr0 -> forall tr1, bisim tr0 tr1 -> p tr1.
 Definition assertS := state -> Prop.
 Definition assertT := { p:  trace -> Prop | setoid p}.
 
@@ -19,63 +19,63 @@ Definition assertS_and (u1 u2: assertS) := fun st =>  u1 st /\ u2 st.
 
 Infix "andS" := assertS_and (at level 60, right associativity).
 
-Definition assertT_and (p1 p2: assertT): assertT. 
-destruct p1 as [f0 h0]. 
-destruct p2 as [f1 h1]. exists (fun tr => f0 tr /\ f1 tr). 
-move => tr0 [h2 h3] tr1 h4. split. 
-* have := h0 _ h2 _ h4; apply. 
+Definition assertT_and (p1 p2: assertT): assertT.
+destruct p1 as [f0 h0].
+destruct p2 as [f1 h1]. exists (fun tr => f0 tr /\ f1 tr).
+move => tr0 [h2 h3] tr1 h4. split.
+* have := h0 _ h2 _ h4; apply.
 * have := h1 _ h3 _ h4; apply.
 Defined.
 
 Infix "andT" := assertT_and (at level 60, right associativity).
 
-Definition assertT_or (p1 p2: assertT): assertT. 
-destruct p1 as [f0 h0]. 
-destruct p2 as [f1 h1]. exists (fun tr => f0 tr \/ f1 tr). 
+Definition assertT_or (p1 p2: assertT): assertT.
+destruct p1 as [f0 h0].
+destruct p2 as [f1 h1]. exists (fun tr => f0 tr \/ f1 tr).
 move => tr0 [h2 | h2] tr1 h3.
-- left. have := h0 _ h2 _ h3; apply. 
-- right. have := h1 _ h2 _ h3; apply. 
+- left. have := h0 _ h2 _ h3; apply.
+- right. have := h1 _ h2 _ h3; apply.
 Defined.
 
 Infix "orT" := assertT_or (at level 60, right associativity).
 
-Definition assertS_imp (u1 u2: assertS) := forall st, u1 st -> u2 st. 
+Definition assertS_imp (u1 u2: assertS) := forall st, u1 st -> u2 st.
 
 Infix "->>" := assertS_imp (at level 60, right associativity).
 
-Lemma assertS_imp_refl: forall u, u ->> u. 
-Proof. 
-move => u st0 h0. done. 
+Lemma assertS_imp_refl: forall u, u ->> u.
+Proof.
+move => u st0 h0. done.
 Qed.
 
-Definition satisfy (p:assertT) (tr: trace): Prop := 
+Definition satisfy (p:assertT) (tr: trace): Prop :=
 let: exist f0 h0 := p in f0 tr.
 
-Definition assertT_imp (p1 p2: assertT) := 
-forall tr, satisfy p1 tr -> satisfy p2 tr.  
+Definition assertT_imp (p1 p2: assertT) :=
+forall tr, satisfy p1 tr -> satisfy p2 tr.
 
 Infix "=>>" := assertT_imp (at level 60, right associativity).
 
 Lemma impT_conseq_L: forall p0 p1 q,
 p0 =>> p1 -> p1 =>> q -> p0 =>> q.
-Proof. move => p0 p1 q. destruct p0 as [p0 hp0]. 
-destruct p1 as [p1 hp1]. destruct q as [q hq]. 
-move => h0 h1 tr0. simpl. move => h2. apply h1. simpl. 
-apply h0. simpl. done. Qed.    
+Proof. move => p0 p1 q. destruct p0 as [p0 hp0].
+destruct p1 as [p1 hp1]. destruct q as [q hq].
+move => h0 h1 tr0. simpl. move => h2. apply h1. simpl.
+apply h0. simpl. done. Qed.
 
 Lemma impT_conseq_R: forall p q0 q1,
 q0 =>> q1 -> p =>> q0 -> p =>> q1.
-Proof. move => p q0 q1. destruct p as [p hp]. 
-destruct q0 as [q0 hq0]. destruct q1 as [q1 hq1]. 
-move => h0 h1 tr0. simpl. move => h2. apply h0. simpl. 
+Proof. move => p q0 q1. destruct p as [p hp].
+destruct q0 as [q0 hq0]. destruct q1 as [q1 hq1].
+move => h0 h1 tr0. simpl. move => h2. apply h0. simpl.
 apply h1. simpl. done. Qed.
 
 Lemma imp_andT: forall p q0 q1,
 p =>> q0 -> p =>> q1 -> p =>> (q0 andT q1).
-Proof. 
+Proof.
 move => [p hp] [q0 hq0] [q1 hq1] h0 h1 tr0 h2.
-simpl in h2. simpl. split. 
-apply h0. done. apply h1. done. 
+simpl in h2. simpl. split.
+apply h0. done. apply h1. done.
 Qed.
 
 Definition ttS: assertS := fun st => True.
@@ -83,26 +83,26 @@ Definition ffS: assertS := fun st => False.
 
 Definition ttt: trace -> Prop := fun tr => True.
 Definition ttT: assertT.
-exists ttt. by move => tr0 h0 tr1 h1. 
+exists ttt. by move => tr0 h0 tr1 h1.
 Defined.
 
-Lemma assertT_imp_refl: forall p, p =>> p. 
-Proof. move => p tr0 h0. done. Qed. 
+Lemma assertT_imp_refl: forall p, p =>> p.
+Proof. move => p tr0 h0. done. Qed.
 
-Lemma satisfy_cont: forall p0 p1, 
+Lemma satisfy_cont: forall p0 p1,
  p0 =>> p1 -> forall tr, satisfy p0 tr -> satisfy p1 tr.
-Proof. move => [f0 h0] [f1 h1] h2 tr h3. 
-simpl. simpl in h3. have := h2 _ h3. apply. 
+Proof. move => [f0 h0] [f1 h1] h2 tr h3.
+simpl. simpl in h3. have := h2 _ h3. apply.
 Qed.
 
 Lemma assertT_imp_trans: forall p q r, p =>> q -> q =>> r -> p =>> r.
-Proof. 
-move => p q r h0 h1 tr0 h2.  
-have := satisfy_cont h1. apply. 
-have := satisfy_cont h0 h2. by apply. 
+Proof.
+move => p q r h0 h1 tr0 h2.
+have := satisfy_cont h1. apply.
+have := satisfy_cont h0 h2. by apply.
 Qed.
 
-Lemma andS_left: forall u1 u2, (u1 andS u2) ->> u1. 
+Lemma andS_left: forall u1 u2, (u1 andS u2) ->> u1.
 Proof. move => u1 u2 st h1; by inversion h1. Qed.
 
 Lemma andS_right: forall u1 u2, (u1 andS u2) ->> u2.
@@ -112,199 +112,200 @@ Lemma andS_cont: forall u1 u1' u2 u2',
 u1 ->> u1' ->
 u2 ->> u2' ->
 (u1 andS u2) ->> (u1' andS u2').
-Proof. 
-move => u1 u1' u2 u2' h1 h2 st [h3 h4]. split. 
-* have := h1 _ h3; apply. 
-* have := h2 _ h4; apply. 
+Proof.
+move => u1 u1' u2 u2' h1 h2 st [h3 h4]. split.
+* have := h1 _ h3; apply.
+* have := h2 _ h4; apply.
 Qed.
 
 Lemma orT_left: forall p1 p2, p1 =>> (p1 orT p2).
 Proof.
 move => p1 p2 tr h1. simpl. destruct p1 as [f1 hf1].
-destruct p2 as [f2 hf2]. simpl. simpl in h1. by left. 
-Qed. 
+destruct p2 as [f2 hf2]. simpl. simpl in h1. by left.
+Qed.
 
 Lemma orT_right: forall p1 p2, p2 =>> (p1 orT p2).
 Proof.
 move => p1 p2 tr h1. simpl. destruct p1 as [f1 hf1].
-destruct p2 as [f2 hf2]. simpl. simpl in h1. by right. 
-Qed. 
+destruct p2 as [f2 hf2]. simpl. simpl in h1. by right.
+Qed.
 
 Definition singleton (u:assertS): trace -> Prop :=
 fun tr => exists st, u st /\ bisim tr (Tnil st).
 
-Lemma singleton_setoid: forall u, setoid (singleton u). 
-Proof. 
-move => u. move => tr0 h0 tr1 h1. move: h0 => [st0 [h0 h2]]. 
-foo h2. foo h1. exists st0. split; [apply h0 | reflexivity]. 
+Lemma singleton_setoid: forall u, setoid (singleton u).
+Proof.
+move => u. move => tr0 h0 tr1 h1. move: h0 => [st0 [h0 h2]].
+inv h2. inv h1. exists st0. split; [apply h0 | reflexivity].
 Qed.
 
 Lemma singleton_monotone: forall u v, u ->> v ->
 forall tr, singleton u tr ->  singleton v tr.
-Proof. 
-move => u v huv tr0 h0. move: h0 => [st0 [h0 h1]]. foo h1. 
-exists st0. split; [ have := huv _ h0; apply | apply bisim_reflexive].
+Proof.
+move => u v huv tr0 h0. move: h0 => [st0 [h0 h1]]. inv h1.
+exists st0. split; [ apply: (huv _ h0) | apply: bisim_reflexive].
 Qed.
 
 Lemma singleton_nil: forall u st,
-singleton u (Tnil st) -> u st. 
-Proof. move => u st [st0 [h0 h1]]. foo h1. done. Qed.
+singleton u (Tnil st) -> u st.
+Proof. move => u st [st0 [h0 h1]]. inv h1. done. Qed.
 
 Lemma mk_singleton_nil: forall (u : state -> Prop) st,
-u st -> singleton u (Tnil st). 
-Proof. move => u st h0. exists st. split; [ done | apply bisim_reflexive]. Qed. 
+u st -> singleton u (Tnil st).
+Proof. move => u st h0. exists st. split=>//; apply bisim_reflexive. Qed.
 
 (* Proposition 3.1: <U> is setoid *)
-Definition Singleton (u: assertS): assertT. 
-exists (singleton u). 
-move => tr0 [st0 [h0 h1]] tr1 h2. foo h1. foo h2.
-exists st0. by split; [done | apply bisim_nil]. 
+Definition Singleton (u: assertS): assertT.
+exists (singleton u).
+move => tr0 [st0 [h0 h1]] tr1 h2. inv h1. inv h2.
+exists st0. by split=>//; apply: bisim_nil.
 Defined.
 
 Notation "[| p |]" := (Singleton p) (at level 80).
 
 (* Proposition 3.2: <U> is monotone *)
 Lemma Singleton_monotone: forall u v,
-u ->> v -> [|u|] =>> [|v|]. 
-Proof. 
-move => u v h0 tr0 h1. move: h1 => [st0 [h1 h2]]. 
-foo h2. exists st0. split; [ have := h0 _ h1; apply | apply bisim_reflexive].
+u ->> v -> [|u|] =>> [|v|].
+Proof.
+move => u v h0 tr0 h1. move: h1 => [st0 [h1 h2]].
+inv h2. exists st0. split; [ apply: (h0 _ h1) | apply: bisim_reflexive].
 Qed.
 
 Definition eval_true (a: expr): assertS  :=
-fun st => is_true (a st) = true. 
+fun st => is_true (a st).
 
 Definition eval_false (a: expr): assertS :=
-fun st => is_true (a st) = false.
+fun st => ~~ is_true (a st).
 
 Definition dup (u: assertS): trace -> Prop :=
 fun tr => exists st, u st /\ bisim tr (Tcons st (Tnil st)).
 
 Lemma dup_cont: forall (u0 u1: assertS),
 u0 ->> u1 ->
-forall tr, dup u0 tr -> dup u1 tr. 
-Proof. 
-move => u0 u1 hu tr [st0 [h0 h1]]. foo h1. foo H1. 
-exists st0. split. have := hu _ h0; apply. reflexivity. 
+forall tr, dup u0 tr -> dup u1 tr.
+Proof.
+move => u0 u1 hu tr [st0 [h0 h1]]. inv h1. inv H1.
+exists st0. split; first by apply: (hu _ h0).
+by apply: bisim_reflexive.
 Qed.
 
 (* Proposition 3.1: <<U>> is setoid *)
-Definition Dup (u: assertS): assertT. 
+Definition Dup (u: assertS): assertT.
 exists (dup u).
-move => tr0 [st0 [h0 h1]] tr1 h2. foo h1. foo H1. foo h2. foo H2. 
-exists st0. split =>//. reflexivity. 
+move => tr0 [st0 [h0 h1]] tr1 h2. inv h1. inv H1. inv h2. inv H2.
+exists st0. split =>//. by apply: bisim_reflexive.
 Defined.
 
 Notation "<< p >>" := (Dup p) (at level 80).
 
 (* Proposition 3.2: <<U>> is monotone *)
 Lemma Dup_monotone: forall u v, u ->> v -> <<u>> =>> <<v>>.
-Proof. move => u v h0 tr0. simpl. apply dup_cont => //. 
+Proof. move => u v h0 tr0. simpl. apply dup_cont => //.
 Qed.
 
 CoInductive follows (p: trace -> Prop): trace -> trace -> Prop :=
 | follows_nil: forall st tr,
   hd tr = st -> p tr ->
-  follows p (Tnil st) tr 
+  follows p (Tnil st) tr
 | follows_delay: forall st tr tr',
   follows p tr tr' -> follows p (Tcons st tr) (Tcons st tr').
 
 Lemma follows_hd: forall p tr0 tr1, follows p tr0 tr1 ->
-hd tr0 = hd tr1. 
-Proof. 
-move => p tr0 tr1 h0. by foo h0; simpl. 
+hd tr0 = hd tr1.
+Proof.
+move => p tr0 tr1 h0. by inv h0; simpl.
 Qed.
 
 Lemma follows_setoid: forall (p: trace -> Prop)
-(hp: forall tr0, p tr0 -> forall tr1, bisim tr0 tr1 -> p tr1), 
+(hp: forall tr0, p tr0 -> forall tr1, bisim tr0 tr1 -> p tr1),
 forall tr0 tr1, follows p tr0 tr1 ->
-forall tr2, bisim tr0 tr2 -> forall tr3, bisim tr1 tr3 -> 
-follows p tr2 tr3. 
-Proof. 
+forall tr2, bisim tr0 tr2 -> forall tr3, bisim tr1 tr3 ->
+follows p tr2 tr3.
+Proof.
 move => p hp. cofix COINDHYP.
-move => tr0 tr1 h0 tr2 h1 tr3 h2. foo h0. 
-- clear COINDHYP. foo h1. have h0 := bisim_hd h2. symmetry in h0. 
-  have := follows_nil h0 (hp _ H0 _ h2). apply. 
-- foo h2. foo h1. have := follows_delay st (COINDHYP _ _ H _ H4 _ H3); apply. 
+move => tr0 tr1 h0 tr2 h1 tr3 h2. inv h0.
+- clear COINDHYP. inv h1. have h0 := bisim_hd h2. symmetry in h0.
+  have := follows_nil h0 (hp _ H0 _ h2). apply.
+- inv h2. inv h1. have := follows_delay st (COINDHYP _ _ H _ H4 _ H3); apply.
 Qed.
 
 Lemma follows_setoid_L: forall p,
 forall tr0 tr1, follows p tr0 tr1 ->
-forall tr2, bisim tr0 tr2 ->  follows p tr2 tr1. 
-Proof. 
-move => p. cofix COINDHYP. move =>  tr tr0 h0 tr1 h1. foo h0. 
-- foo h1. apply follows_nil. reflexivity. apply H0. 
-- foo h1. have := follows_delay st (COINDHYP _ _ H _ H3). apply. 
+forall tr2, bisim tr0 tr2 ->  follows p tr2 tr1.
+Proof.
+move => p. cofix COINDHYP. move =>  tr tr0 h0 tr1 h1. inv h0.
+- inv h1. apply follows_nil. reflexivity. apply H0.
+- inv h1. have := follows_delay st (COINDHYP _ _ H _ H3). apply.
 Qed.
 
 Lemma follows_setoid_R: forall (p: trace -> Prop)
-(hp: forall tr0, p tr0 -> forall tr1, bisim tr0 tr1 -> p tr1), 
+(hp: forall tr0, p tr0 -> forall tr1, bisim tr0 tr1 -> p tr1),
 forall tr tr0, follows p tr tr0 ->
-forall tr1, bisim tr0 tr1 ->  follows p tr tr1. 
-Proof. 
-move => p hp. cofix COINDHYP. 
-move => tr tr0 h0 tr1 h1. foo h0.  
-- apply follows_nil. symmetry. have := bisim_hd h1. apply. 
-  have := hp _ H0 _ h1; apply.  
-- foo h1. have := follows_delay st (COINDHYP _ _  H _ H3). apply.
+forall tr1, bisim tr0 tr1 ->  follows p tr tr1.
+Proof.
+move => p hp. cofix COINDHYP.
+move => tr tr0 h0 tr1 h1. inv h0.
+- apply follows_nil. symmetry. have := bisim_hd h1. apply.
+  have := hp _ H0 _ h1; apply.
+- inv h1. have := follows_delay st (COINDHYP _ _  H _ H3). apply.
 Qed.
 
 Lemma follows_monotone: forall (p q : trace -> Prop),
-(forall tr, p tr -> q tr) -> 
+(forall tr, p tr -> q tr) ->
 forall tr0 tr1, follows p tr0 tr1 -> follows q tr0 tr1.
-Proof. 
-move => p q hpq. cofix hcoind. move => tr0 tr1 h0. foo h0. 
+Proof.
+move => p q hpq. cofix hcoind. move => tr0 tr1 h0. inv h0.
 - apply follows_nil => //. have := hpq _ H0; by apply.
-- have := follows_delay _ (hcoind _ _ H). by apply. 
-Qed.    
+- have := follows_delay _ (hcoind _ _ H). by apply.
+Qed.
 
 (* Lemma 3.2 *)
-Lemma follows_singleton: forall u tr0 tr1, 
+Lemma follows_singleton: forall u tr0 tr1,
 follows (singleton u) tr0 tr1 -> bisim tr0 tr1.
-Proof. 
-move => u. cofix COINDHYP. move => tr0 tr1 h0. foo h0. 
-- move: H0 => [st0 [h0 h1]]. foo h1. by simpl; apply bisim_reflexive.  
+Proof.
+move => u. cofix COINDHYP. move => tr0 tr1 h0. inv h0.
+- move: H0 => [st0 [h0 h1]]. inv h1. by simpl; apply bisim_reflexive.
 - have := bisim_cons st (COINDHYP _ _ H); apply.
 Qed.
 
 Lemma follows_singleton_andS_L: forall u0 u1 tr0,
 follows (singleton (u0 andS u1)) tr0 tr0 ->
 follows (singleton u0) tr0 tr0.
-Proof. 
-move => u0 u1. cofix hcoind. case. 
+Proof.
+move => u0 u1. cofix hcoind. case.
 - move => st0 h0. inversion h0. clear H1 H. simpl in H0.
-  foo h0.
-  move: H3 => [st1 [h1 h2]]. foo h2. move: h1 => [h1 h2].
+  inv h0.
+  move: H3 => [st1 [h1 h2]]. inv h2. move: h1 => [h1 h2].
   apply follows_nil => //. exists st1. split; [done | apply bisim_reflexive].
-- move => st0 tr0 h0. foo h0. 
-  have := follows_delay st0 (hcoind _ H0). by apply. 
-Qed. 
+- move => st0 tr0 h0. inv h0.
+  have := follows_delay st0 (hcoind _ H0). by apply.
+Qed.
 
 Lemma follows_singleton_andS_R: forall u0 u1 tr0,
 follows (singleton (u0 andS u1)) tr0 tr0 ->
 follows (singleton u1) tr0 tr0.
-Proof. 
-move => u0 u1. cofix hcoind. case. 
+Proof.
+move => u0 u1. cofix hcoind. case.
 - move => st0 h0. inversion h0. clear H1 H. simpl in H0.
-  foo h0.
-  move: H3 => [st1 [h1 h2]]. foo h2. move: h1 => [h1 h2].
+  inv h0.
+  move: H3 => [st1 [h1 h2]]. inv h2. move: h1 => [h1 h2].
   apply follows_nil => //. exists st1. split; [done | apply bisim_reflexive].
-- move => st0 tr0 h0. foo h0. 
-  have := follows_delay st0 (hcoind _ H0). by apply. 
-Qed. 
-     
+- move => st0 tr0 h0. inv h0.
+  have := follows_delay st0 (hcoind _ H0). by apply.
+Qed.
+
 Lemma singleton_andS_follows: forall u v tr,
 follows (singleton u) tr tr -> follows (singleton v) tr tr ->
-follows (singleton (u andS v)) tr tr. 
-Proof. 
+follows (singleton (u andS v)) tr tr.
+Proof.
 move => u v. cofix hcoind. move => tr h0 h1. inversion h0; subst.
-- apply follows_nil => //. exists st. split; last by apply bisim_reflexive. 
+- apply follows_nil => //. exists st. split; last by apply bisim_reflexive.
   clear H. inversion h1; subst. clear H1.
   have := singleton_nil H0.
   have := singleton_nil H2.
   by split.
-- subst. foo h0. foo h1. have := follows_delay st (hcoind _ H1 H2); by apply. 
-Qed.  
+- subst. inv h0. inv h1. have := follows_delay st (hcoind _ H1 H2); by apply.
+Qed.
 
 CoFixpoint lastdup (tr: trace): trace :=
 match tr with
@@ -312,22 +313,22 @@ match tr with
 | Tcons st tr' => Tcons st (lastdup tr')
 end.
 
-Lemma lastdup_hd: forall tr, hd tr = hd (lastdup tr). 
-Proof. 
-case. 
+Lemma lastdup_hd: forall tr, hd tr = hd (lastdup tr).
+Proof.
+case.
 - move => st. rewrite [lastdup _]trace_destr. by simpl.
 - move => st tr. rewrite [lastdup _]trace_destr. by simpl.
 Qed.
 
 Lemma follows_dup: forall u tr, follows (singleton u) tr tr ->
-follows (dup u) tr (lastdup tr). 
+follows (dup u) tr (lastdup tr).
 Proof.
-move => u. cofix COINDHYP. move => tr0 h0. inversion h0. 
-- clear H H1 H2 h0. rewrite [lastdup _]trace_destr. simpl. 
-  move: H0 => [st1 [h0 h1]]. foo h1. apply follows_nil => //. exists st1.
-  split; [done | reflexivity]. 
-- clear h0 H0 H. rewrite [lastdup _]trace_destr. simpl. 
-  have := follows_delay st (COINDHYP _ H1). apply. 
+move => u. cofix COINDHYP. move => tr0 h0. inversion h0.
+- clear H H1 H2 h0. rewrite [lastdup _]trace_destr. simpl.
+  move: H0 => [st1 [h0 h1]]. inv h1. apply follows_nil => //. exists st1.
+  split; [done | reflexivity].
+- clear h0 H0 H. rewrite [lastdup _]trace_destr. simpl.
+  have := follows_delay st (COINDHYP _ H1). apply.
 Qed.
 
 Definition append (p1 p2: trace -> Prop ): trace -> Prop :=
@@ -338,45 +339,45 @@ Infix "*+*" := append (at level 60, right associativity).
 Lemma append_cont: forall (p0 p1 q0 q1: trace -> Prop),
 (forall tr, p0 tr -> p1 tr) ->
 (forall tr, q0 tr -> q1 tr) ->
-forall tr, append p0 q0 tr -> append p1 q1 tr. 
-Proof. 
+forall tr, append p0 q0 tr -> append p1 q1 tr.
+Proof.
 move => p0 p1 q0 q1 hp hq tr [tr0 [h0 h1]].
-exists tr0. split. have := hp _ h0; apply. clear h0. 
-move: tr0 tr h1. cofix COINDHYP. 
-move => tr0 tr1 h0. foo h0.
-- apply follows_nil => //. have := hq _ H0; apply. 
-- have := follows_delay st (COINDHYP _ _ H); apply. 
+exists tr0. split. have := hp _ h0; apply. clear h0.
+move: tr0 tr h1. cofix COINDHYP.
+move => tr0 tr1 h0. inv h0.
+- apply follows_nil => //. have := hq _ H0; apply.
+- have := follows_delay st (COINDHYP _ _ H); apply.
 Qed.
 
 Lemma append_cont_L: forall (p0 p1 q: trace -> Prop),
 (forall tr, p0 tr -> p1 tr) ->
 forall tr, (append p0 q tr) -> (append p1 q tr).
-Proof. 
-move => p0 p1 q hp. move => tr [tr0 [h0 h1]]. 
-exists tr0. split. have := hp _ h0; apply. apply h1. 
+Proof.
+move => p0 p1 q hp. move => tr [tr0 [h0 h1]].
+exists tr0. split. have := hp _ h0; apply. apply h1.
 Qed.
 
 Lemma append_monotone_R: forall (p q0 q1: trace -> Prop),
 (forall tr, q0 tr -> q1 tr) ->
 forall tr, (append p q0 tr) -> (append p q1 tr).
-Proof. 
+Proof.
 move => p q0 q1 hq. have := (@append_cont p p _ _ _ hq). apply => //.
 Qed.
 
 Lemma append_setoid: forall (p0 p1: trace -> Prop),
-setoid p1 -> setoid (append p0 p1). 
-Proof. 
+setoid p1 -> setoid (append p0 p1).
+Proof.
 move => p0 p1 hp1. move => tr0 h0 tr1 h1.
 move: h0 => [tr2 [h0 h2]]. exists tr2. split; first by apply h0.
-have := follows_setoid_R hp1 h2 h1. apply. 
+have := follows_setoid_R hp1 h2 h1. apply.
 Qed.
 
 Lemma follows_follows: forall p q tr0 tr1 tr2, follows p tr0 tr1 ->
-follows q tr1 tr2 -> follows (p *+* q) tr0 tr2. 
+follows q tr1 tr2 -> follows (p *+* q) tr0 tr2.
 Proof. move => p q. cofix hcoind. case.
-- move => st0 tr1 tr2 h0 h1. foo h0. have := follows_hd h1 => h2. 
-  apply follows_nil => //. exists tr1. split => //. 
-- move => st0 tr0 tr1 tr2 h0 h1. foo h0. foo h1. apply follows_delay. 
+- move => st0 tr1 tr2 h0 h1. inv h0. have := follows_hd h1 => h2.
+  apply follows_nil => //. exists tr1. split => //.
+- move => st0 tr0 tr1 tr2 h0 h1. inv h0. inv h1. apply follows_delay.
   have := hcoind _ _ _ H2 H3. apply.
 Qed.
 
@@ -393,194 +394,208 @@ midp h tr' ->
 follows p0 tr0 tr'.
 Proof.
 cofix COINDHYP. dependent inversion h. move => {tr H0}.
-- move: tr1 st tr0 h e a H. case. 
-  - move => st0 st1 tr0 h1 h2 h3 h4. simpl in h2.  
+- move: tr1 st tr0 h e a H. case.
+  - move => st0 st1 tr0 h1 h2 h3 h4. simpl in h2.
     move => tr' hm.
-    foo hm; last by inversion H.
-    destruct h3. destruct H2. inversion h1. 
+    inv hm; last by inversion H.
+    destruct h3. destruct H2. inversion h1.
     subst. apply follows_nil; last by [].
     by inversion H1.
   - move => st0 tr0 st1 tr1 h1 h2 h3 h4. simpl in h2.
     move => tr' hm.
-    foo hm; last by inversion H.
+    inv hm; last by inversion H.
     destruct h3. destruct H2. inversion h1.
-    subst. apply follows_nil; last by []. by inversion H1. 
-- subst. 
+    subst. apply follows_nil; last by []. by inversion H1.
+- subst.
   move => tr0 hm.
   destruct tr0; first by inversion hm.
-  foo hm; subst; first by inversion H.
-  foo H1; subst.
-  foo H2; subst.
-  apply follows_delay. 
-  by have := COINDHYP _ _ _ _ h1; apply. 
+  inv hm; subst; first by inversion H.
+  inv H1; subst.
+  inv H2; subst.
+  apply follows_delay.
+  by have := COINDHYP _ _ _ _ h1; apply.
 Qed.
 
 Lemma midp_after: forall p0 p1 tr0 tr1 (h: follows (append p0 p1) tr0 tr1) tr',
 midp h tr' ->
 follows p1 tr' tr1.
 Proof.
-cofix COINDHYP. dependent inversion h. move => {tr H0}. 
-- move: tr1 st tr0 h e a H. case. 
+cofix COINDHYP. dependent inversion h. move => {tr H0}.
+- move: tr1 st tr0 h e a H. case.
   * move => st0 st1 tr0 h1 h2 h3 h4. simpl in h2. move => tr' hm.
-    foo hm; last by inversion H. destruct tr'; last by inversion H. destruct h3. destruct H2. inversion H3. subst.
-    apply follows_nil; last by []. by inversion H1. 
+    inv hm; last by inversion H. destruct tr'; last by inversion H. destruct h3. destruct H2. inversion H3. subst.
+    apply follows_nil; last by []. by inversion H1.
   * move => st0 tr0 st1 tr1 h1 h2 h3 h4. simpl in h2.
-    move => tr' hm. by foo hm; last by inversion H.
-- subst. 
+    move => tr' hm. by inv hm; last by inversion H.
+- subst.
   move => tr0 hm.
  destruct tr0; first by inversion hm.
- foo hm; subst; first by inversion H.
- foo H1; subst.
- foo H2; subst.
+ inv hm; subst; first by inversion H.
+ inv H1; subst.
+ inv H2; subst.
  apply follows_delay.
- by have := COINDHYP _ _ _ _ h1; apply. 
+ by have := COINDHYP _ _ _ _ h1; apply.
 Qed.
 
 Lemma append_assoc_L: forall p1 p2 p3 tr,
 (append (append p1 p2) p3) tr -> append p1 (append p2  p3) tr.
-Proof. 
+Proof.
 move => p1 p2 p3 tr0 h1. move: h1 => [tr1 [h1 h2]]. move: h1 => [tr2 h1].
-move: h1 => [h1 h3]. exists tr2. split; first done. clear h1.  
-move: tr2 tr0 tr1 h2 h3. cofix COINDHYP. move => tr0 tr1 tr2 h1 h2. foo h2. 
-- have h2 := follows_hd h1. symmetry in h2. have := follows_nil h2.  apply. 
-  exists tr2. by split. 
-- foo h1. apply follows_delay. have := COINDHYP _ _ _ H3 H; apply. 
-Qed. 
+move: h1 => [h1 h3]. exists tr2. split; first done. clear h1.
+move: tr2 tr0 tr1 h2 h3. cofix COINDHYP. move => tr0 tr1 tr2 h1 h2. inv h2.
+- have h2 := follows_hd h1. symmetry in h2. have := follows_nil h2.  apply.
+  exists tr2. by split.
+- inv h1. apply follows_delay. have := COINDHYP _ _ _ H3 H; apply.
+Qed.
 
 (* Proposition 3.1: ** is setoid. *)
-Definition Append (p1 p2: assertT): assertT.  
-destruct p1 as [f0 h0]. 
-destruct p2 as [f1 h1]. exists (append f0 f1).  
+Definition Append (p1 p2: assertT): assertT.
+destruct p1 as [f0 h0].
+destruct p2 as [f1 h1]. exists (append f0 f1).
 move => tr0 [tr1 [h2 h3]] tr2 h4. exists tr1.
-split. apply h2.  have := follows_setoid_R h1 h3 h4. apply.  
-Defined. 
+split. apply h2.  have := follows_setoid_R h1 h3 h4. apply.
+Defined.
 
 Infix "***" := Append (at level 60, right associativity).
 
 (* Lemma 3.4 (4) => *)
 Lemma Append_assoc_L: forall p1 p2 p3,
 ((p1 *** p2) *** p3) =>> (p1 *** p2 *** p3).
-Proof. 
-move => p1 p2 p3 tr0 h1. destruct p1 as [f1 hf1]. destruct p2 as [f2 hf2]. 
-destruct p3 as [f3 hf3]. simpl. simpl in h1. have := append_assoc_L h1. apply. 
+Proof.
+move => [f1 hf1] [f2 hf2] [f3 hf3] tr0 /= h1.
+by apply: append_assoc_L.
 Qed.
 
 (* Proposition 3.2: ** is monotone *)
 Lemma Append_monotone: forall p1 p2 q1 q2,
-p1 =>> p2 -> q1 =>> q2 -> (p1 *** q1) =>> (p2 *** q2). 
-Proof. move => p1 p2 q1 q2 h0 h1. destruct p1 as [p1 hp1]. destruct p2 as [p2 hp2].
-destruct q1 as [q1 hq1]. destruct q2 as [q2 hq2].  move => tr0. simpl. 
-move => h2. have := append_cont _ _ h2. apply. apply h0. apply h1. 
-Qed.   
+p1 =>> p2 -> q1 =>> q2 -> (p1 *** q1) =>> (p2 *** q2).
+Proof.
+move=> [p1 hp1] [p2 hp2] [q1 hq1] [q2 hq2] h0 h1 tr0 /= h2.
+by apply: (append_cont _ _ h2).
+Qed.
 
 Lemma Append_monotone_L: forall p1 p2 q,
-p1 =>> p2 -> (p1 *** q) =>> (p2 *** q). 
-Proof. 
-move => p1 p2 q h0. destruct p1 as [p1 hp1]. destruct p2 as [p2 hp2].
-destruct q as [q hq]. move => tr0. simpl.  
-have := append_cont_L h0.  apply.
-Qed.   
+p1 =>> p2 -> (p1 *** q) =>> (p2 *** q).
+Proof.
+move=> [p1 hp1] [p2 hp2] [q hq] h0 tr0 /=.
+by apply: append_cont_L.
+Qed.
 
 Lemma Append_monotone_R: forall q p1 p2,
-p1 =>> p2 -> (q *** p1) =>> (q *** p2). 
-Proof. 
-move => q p1 p2 h0. destruct p1 as [p1 hp1]. destruct p2 as [p2 hp2].
-destruct q as [q hq]. move => tr0. simpl. move => h1.   
-have := (@append_cont q q p1 p2). apply. done. apply h0. 
-exact h1.
+p1 =>> p2 -> (q *** p1) =>> (q *** p2).
+Proof.
+move => [q hq] [p1 hp1] [p2 hp2] h0 tr0 /= h1.
+by apply: (@append_cont q q p1 p2).
 Qed.
 
 Lemma Append_ttS: forall p,
-p =>> (p *** [| ttS |]). 
+p =>> (p *** [| ttS |]).
 Proof.
-move => [f hp] tr0 h0. simpl in h0. simpl. exists tr0. 
-split; first done. clear h0 hp. move: tr0. cofix hcoind. 
-case. move => st0. apply follows_nil => //.
-by apply mk_singleton_nil. move => st0 tr0. 
-have := follows_delay _ (hcoind _). by apply. 
+move => [f hp] tr0 /= h0. exists tr0.
+split=>// {h0 hp}. move: tr0. cofix hcoind.
+case=>st0.
+- apply: follows_nil => //; by apply mk_singleton_nil.
+move=>tr0.
+by apply/follows_delay/hcoind.
 Qed.
 
 (* Lemma 3.4 (1), the first => *)
 Lemma Sglt_Dup_1: forall u v, ([|u|] *** <<v>>) =>> <<u andS v>>.
-Proof. move => u v tr0 [tr1 [h0 h1]]. simpl. destruct h0 as [st0 [h0 h2]]. foo h2. 
-foo h1. destruct H1 as [st0 [h1 h2]]. foo h2. foo H1. simpl in h0. exists st0. 
-split; last by apply bisim_reflexive. by split. Qed. 
+Proof.
+move=>u v tr0 [tr1 [[st0 [h0 h2]] h1]] /=. inv h2. inv h1.
+destruct H1 as [st0 [h1 h2]]. inv h2. inv H1. simpl in h0. exists st0.
+by split=>//; apply: bisim_reflexive.
+Qed.
 
 (* Lemma 3.4 (1), the first <= *)
-Lemma Sglt_Dup_2: forall u v, <<u andS v>> =>> ([|u|] *** <<v>>). 
-Proof. move => u v tr0 [st0 [[hu hv] h1]]. foo h1. foo H1. exists (Tnil st0). split. 
-* exists st0. by split; last apply bisim_reflexive.
-* apply follows_nil => //. exists st0. by split; last apply bisim_reflexive. 
-Qed. 
+Lemma Sglt_Dup_2: forall u v, <<u andS v>> =>> ([|u|] *** <<v>>).
+Proof.
+move => u v tr0 [st0 [[hu hv] h1]]. inv h1. inv H1. exists (Tnil st0). split.
+* exists st0. by split=>//; apply: bisim_reflexive.
+* apply follows_nil => //. exists st0. by split=>//; apply: bisim_reflexive.
+Qed.
 
 (* Lemma 3.4 (1), the second => *)
-Lemma Sglt_Dup_3: forall u v, <<u andS v>> =>> <<u>> *** [|v|]. 
-Proof. move => u v tr0 [st0 [[hu hv] h0]]. foo h0. foo H1. exists (Tcons st0 (Tnil st0)). 
-split. exists st0. by split; last apply bisim_reflexive. apply follows_delay.
-apply follows_nil => //. exists st0. by split; last apply bisim_reflexive.
-Qed. 
+Lemma Sglt_Dup_3: forall u v, <<u andS v>> =>> <<u>> *** [|v|].
+Proof.
+move => u v tr0 [st0 [[hu hv] h0]]. inv h0. inv H1. exists (Tcons st0 (Tnil st0)).
+split.
+- exists st0. by split=>//; apply: bisim_reflexive.
+apply/follows_delay/follows_nil => //. exists st0.
+by split=>//; apply: bisim_reflexive.
+Qed.
 
 (* Lemma 3.4 (1), the second <= *)
 Lemma Sglt_Dup_4: forall u v, (<<u>> *** [|v|]) =>> <<u andS v>>.
-Proof. move => u v tr0 [tr1 [h0 h1]]. destruct h0 as [st0 [hu h0]]. foo h0. foo H1. 
-foo h1. foo H2. destruct H1 as [st0 [hv h0]]. foo h0. simpl in hu. simpl. 
-exists st0. by split; last apply bisim_reflexive. 
-Qed.       
+Proof.
+move => u v tr0 [tr1 [[st0 [hu h0]] h1]]. inv h0. inv H1.
+inv h1. inv H2. destruct H1 as [st0 [hv h0]]. inv h0. simpl in hu. simpl.
+exists st0. by split=>//; apply: bisim_reflexive.
+Qed.
 
 (* Lemma 3.4 (2), => *)
-Lemma Sglt_Chop_1: forall u v, ([|u|] *** [|v|]) =>> [|u andS v|]. 
-Proof. move => u v tr0 [tr1 [h0 h1]]. destruct h0 as [st0 [hu h0]]. foo h0. 
-foo h1. destruct H1 as [st0 [hv h0]]. foo h0. simpl in hu. exists st0. 
-by split; last apply bisim_reflexive. Qed. 
+Lemma Sglt_Chop_1: forall u v, ([|u|] *** [|v|]) =>> [|u andS v|].
+Proof.
+move => u v tr0 [tr1 [[st0 [hu h0]] h1]]. inv h0.
+inv h1. destruct H1 as [st0 [hv h0]]. inv h0. simpl in hu. exists st0.
+by split=>//; apply: bisim_reflexive.
+Qed.
 
 (* Lemma 3.4 (2), <= *)
-Lemma Sglt_Chop_2: forall u v, [|u andS v|] =>> [|u|] *** [|v|]. 
-Proof. move => u v tr0 [st0 [[hu hv] h0]]. foo h0. exists (Tnil st0). 
-split. exists st0. by split; last apply bisim_reflexive. apply follows_nil => //. 
-exists st0. by split; last apply bisim_reflexive. Qed.
+Lemma Sglt_Chop_2: forall u v, [|u andS v|] =>> [|u|] *** [|v|].
+Proof.
+move => u v tr0 [st0 [[hu hv] h0]]. inv h0. exists (Tnil st0).
+split.
+- exists st0. by split=>//; apply: bisim_reflexive.
+apply: follows_nil => //.
+exists st0. by split=>//; apply: bisim_reflexive.
+Qed.
 
-Lemma Singleton_Append: forall v p, ([|v|] *** p) =>> p. 
-Proof. move => v [p hp] tr0. simpl. move => [tr1 [h0 h1]]. 
-destruct h0 as [st0 [h0 h2]]. foo h2. foo h1. done. Qed.
+Lemma Singleton_Append: forall v p, ([|v|] *** p) =>> p.
+Proof.
+move => v [p hp] tr0 /= [tr1 [[st0 [h0 h2]] h1]].
+inv h2. by inv h1.
+Qed.
 
 (* Lemma 3.4 (3), the first => *)
 Lemma ttS_Chop: forall p,
 ([|ttS|] *** p) =>> p.
-Proof. move => p. by apply Singleton_Append. Qed. 
+Proof. move => p. by apply Singleton_Append. Qed.
 
 (* Lemma 3.4 (3), the first <= *)
 Lemma ttS_Chop_2: forall p,  p =>> [|ttS|] *** p.
-Proof. move => [p hp] tr0; simpl => htr0. exists (Tnil (hd tr0)). split. 
-exists (hd tr0). by split; last apply bisim_reflexive. 
-apply follows_nil => //. Qed.      
-
-Lemma append_singleton: forall p (hp: setoid p) u tr, 
-append p (singleton u) tr -> p tr.
-Proof. 
-move => p hp u tr0 h1. move: h1 => [tr1 [h1 h2]].
-have h3 := follows_singleton h2. 
-have := hp _ h1 _ h3. apply.
+Proof.
+move => [p hp] tr0 /= htr0. exists (Tnil (hd tr0)). split.
+- exists (hd tr0). by split=>//; apply: bisim_reflexive.
+by exact: follows_nil.
 Qed.
 
-Lemma Append_Singleton: forall p v, (p *** [|v|]) =>> p. 
-Proof. move => [p hp] v tr0. simpl. by apply append_singleton. Qed. 
+Lemma append_singleton: forall p (hp: setoid p) u tr,
+append p (singleton u) tr -> p tr.
+Proof.
+move => p hp u tr0 [tr1 [h1 h2]].
+have h3 := follows_singleton h2.
+apply: (hp _ h1 _ h3).
+Qed.
+
+Lemma Append_Singleton: forall p v, (p *** [|v|]) =>> p.
+Proof. move => [p hp] v tr0 /=. by apply append_singleton. Qed.
 
 (* Lemma 3.4 (3), the second <= *)
 Lemma Chop_ttS: forall p, (p *** [|ttS|]) =>> p.
-Proof. move => p. by apply Append_Singleton. Qed. 
+Proof. move => p. by apply Append_Singleton. Qed.
 
 (* Lemma 3.4 (3), the second => *)
 Lemma Chop_ttS_2: forall p, p =>> p *** [|ttS|].
-Proof. move => [p hp] tr0; simpl => htr0. exists tr0; split; first done. 
-clear hp htr0. move: tr0. cofix hcoind. case. 
-- move => st0. apply follows_nil => //. exists st0. by split; last apply bisim_reflexive. 
-- move => st0 tr0. have := follows_delay _ (hcoind _). apply. 
-Qed. 
-
-Lemma ttT_idem_comp: (ttT *** ttT) =>> ttT. 
 Proof.
-move => tr _. done. 
+move => [p hp] tr0 /= htr0. exists tr0; split=>// {hp htr0}.
+move: tr0. cofix hcoind. case=>st0.
+- apply follows_nil=>//. exists st0. by split=>//; apply: bisim_reflexive.
+- by move=>tr0; apply/follows_delay/hcoind.
 Qed.
+
+Lemma ttT_idem_comp: (ttT *** ttT) =>> ttT.
+Proof. by []. Qed.
 
 Inductive finite: trace -> Prop :=
 | finite_nil: forall st, finite (Tnil st)
@@ -588,108 +603,111 @@ Inductive finite: trace -> Prop :=
   finite tr -> finite (Tcons st tr).
 
 Lemma finite_setoid: forall tr, finite tr ->
-forall tr0, bisim tr tr0 -> finite tr0. 
-Proof. 
-induction 1. 
-- move => tr0 h0. foo h0. apply finite_nil. 
-- move => tr0 h0. foo h0. have := finite_delay st (IHfinite _ H3). 
-  by apply. 
-Qed. 
-
-(* Proposition 3.1: finite is setoid. *)
-Definition Finite: assertT. 
-exists (fun tr => finite tr). 
-move => tr0 h0 tr1 h1. have := finite_setoid h0 h1. apply.
-Defined.     
-
-Lemma Finite_idem_1: (Finite *** Finite) =>> Finite.
-Proof. move => tr0 [tr1 [h0 h1]]. move: tr1 h0 tr0 h1. induction 1. 
-  - move => tr0 h0. foo h0. done. 
-  - move => tr0 h1. foo h1. have h1 := IHh0 _ H2.
-    have := finite_delay _ h1. by apply. Qed. 
-
-Lemma Finite_idem_2: Finite =>> Finite *** Finite. 
-Proof. move => tr0 h0. simpl. exists (Tnil (hd tr0)). split. 
-apply finite_nil. apply follows_nil => //.     
+forall tr0, bisim tr tr0 -> finite tr0.
+Proof.
+induction 1=>tr0 h0; inv h0.
+- by apply: finite_nil.
+- by apply/finite_delay/IHfinite.
 Qed.
 
-Lemma Finite_singleton: forall u, (Finite *** [|u|]) =>> Finite. 
-Proof. 
-move => u tr h0. simpl in h0. simpl. 
-move: h0 => [tr1 [h0 h1]]. 
-have h2 := follows_singleton h1 => {h1}.
-have := finite_setoid h0 h2. by apply. 
+(* Proposition 3.1: finite is setoid. *)
+Definition Finite: assertT.
+exists (fun tr => finite tr).
+move => tr0 h0 tr1 h1.
+apply: (finite_setoid h0 h1).
+Defined.
+
+Lemma Finite_idem_1: (Finite *** Finite) =>> Finite.
+Proof.
+move => tr0 [tr1 [h0 h1]]. move: tr1 h0 tr0 h1. induction 1=>tr0.
+- move => h0. by inv h0.
+- move => h1. inv h1.
+  by apply/finite_delay/IHh0.
+Qed.
+
+Lemma Finite_idem_2: Finite =>> Finite *** Finite.
+Proof.
+move => tr0 h0 /=; exists (Tnil (hd tr0)).
+by split; [apply: finite_nil|apply: follows_nil].
+Qed.
+
+Lemma Finite_singleton: forall u, (Finite *** [|u|]) =>> Finite.
+Proof.
+move => u tr /= [tr1 [h0 h1]].
+by apply/(finite_setoid h0)/follows_singleton/h1.
 Qed.
 
 CoInductive iter (p: trace -> Prop): trace -> Prop :=
 | iter_stop: forall st, iter p (Tnil st)
-| iter_loop: forall tr tr0, 
+| iter_loop: forall tr tr0,
   p tr ->
   follows (iter p) tr tr0 ->
   iter p tr0.
 
-Lemma iter_setoid: forall p (hp: setoid p), setoid (iter p). 
-Proof. 
-move => p hp. cofix COINDHYP.  
+Lemma iter_setoid: forall p (hp: setoid p), setoid (iter p).
+Proof.
+move => p hp. cofix COINDHYP.
 have h0: forall tr, setoid (follows (iter p) tr).
-* cofix COINDHYP1. move => tr. move => tr0 h0 tr1 h1. foo h0. 
-  - apply follows_nil. symmetry. have := bisim_hd h1. apply. 
-    have := COINDHYP _ H0 _ h1. apply.  
-  - foo h1. have := follows_delay st (COINDHYP1 _ _ H _ H3). apply.
-* move => tr0 h1 tr1 h2. foo h1. 
-  - foo h2. apply iter_stop. 
-  - have := iter_loop H (h0 _ _ H0 _ h2). apply. 
+* cofix COINDHYP1. move => tr. move => tr0 h0 tr1 h1. inv h0.
+  - apply: follows_nil; first by apply/esym/bisim_hd.
+    by apply: (COINDHYP _ H0 _ h1).
+  - inv h1. apply: (follows_delay st (COINDHYP1 _ _ H _ H3)).
+* move => tr0 h1 tr1 h2. inv h1.
+  - inv h2. by apply: iter_stop.
+  - by apply: (iter_loop H (h0 _ _ H0 _ h2)).
 Qed.
 
 Lemma iter_cont: forall (p0 p1: trace -> Prop),
 (forall tr, p0 tr -> p1 tr) ->
-forall tr, iter p0 tr -> iter p1 tr. 
-Proof. 
-move => p0 p1 hp. cofix COINDHYP. 
+forall tr, iter p0 tr -> iter p1 tr.
+Proof.
+move => p0 p1 hp. cofix COINDHYP.
 have h: forall tr0 tr1, follows (iter p0) tr0 tr1 -> follows (iter p1) tr0 tr1.
-* cofix COINDHYP0. move => tr0 tr1 h0. foo h0. 
-  - apply follows_nil. reflexivity. have := COINDHYP _ H0; apply. 
-  - have := follows_delay st (COINDHYP0 _ _ H). apply. 
-* move => tr0 h0. foo h0. 
-  - apply iter_stop. 
-  - have := iter_loop (hp _ H)  (h _ _ H0). apply. 
+* cofix COINDHYP0. move => tr0 tr1 h0. inv h0.
+  - apply follows_nil. reflexivity. have := COINDHYP _ H0; apply.
+  - have := follows_delay st (COINDHYP0 _ _ H). apply.
+* move => tr0 h0. inv h0.
+  - apply iter_stop.
+  - have := iter_loop (hp _ H)  (h _ _ H0). apply.
 Qed.
 
 Lemma iter_append_dup: forall (u : state -> Prop) p tr,
 u (hd tr) -> iter (append p (dup u)) tr ->
-follows (singleton u) tr tr. 
-Proof. 
-move => u p.  cofix hcoind. move => tr h0 h1. foo h1. 
-- simpl in h0. apply follows_nil => //. exists st. 
-  by split; [done | apply bisim_reflexive]. 
+follows (singleton u) tr tr.
+Proof.
+move => u p.  cofix hcoind. move => tr h0 h1. inv h1.
+- simpl in h0. apply follows_nil => //. exists st.
+  by split; [done | apply bisim_reflexive].
 - move: H => [tr1 [h2 h1]]. clear h2 h0. (*
   have h2 := follows_hd X0.  rewrite -h2 in h0 => {h2}.   *)
-  move: tr tr1 tr0 h1 H0. cofix hcoind1. 
-  move => tr0 tr1 tr2 h0 h1. foo h0.
-  - move: H0 => [st0 [h0 h3]]. foo h3. foo H1. 
-    foo h1. foo H2. have := follows_delay _ (hcoind _ h0 H1). by apply.  
-  - foo h1. have := follows_delay _ (hcoind1 _ _ _ H H3). by apply. 
-Qed. 
+  move: tr tr1 tr0 h1 H0. cofix hcoind1.
+  move => tr0 tr1 tr2 h0 h1. inv h0.
+  - move: H0 => [st0 [h0 h3]]. inv h3. inv H1.
+    inv h1. inv H2. have := follows_delay _ (hcoind _ h0 H1). by apply.
+  - inv h1. have := follows_delay _ (hcoind1 _ _ _ H H3). by apply.
+Qed.
 
 (* Proposition 3.2: Iter is setoid. *)
-Definition Iter (p: assertT): assertT. 
-destruct p as [f0 h0].  exists (iter f0). apply iter_setoid. apply h0. 
+Definition Iter (p: assertT): assertT.
+destruct p as [f0 h0].  exists (iter f0). apply iter_setoid. apply h0.
 Defined.
 
 (* Proposition 3.2: Iter is monotone. *)
-Lemma Iter_monotone: forall p q, p =>> q -> (Iter p) =>> (Iter q). 
-Proof. move => p q h0 tr0. destruct p as [p hp]. destruct q as [q hq]. 
-simpl. apply iter_cont. move => tr1. apply h0. Qed.
+Lemma Iter_monotone: forall p q, p =>> q -> (Iter p) =>> (Iter q).
+Proof.
+move => [p hp] [q hq] h0 tr0 /=.
+apply: iter_cont=> tr1. apply: h0.
+Qed.
 
-Definition updt (u: assertS) (x:id) (a: expr): trace -> Prop := 
+Definition updt (u: assertS) (x:id) (a: expr): trace -> Prop :=
 fun tr => exists st, u st /\ bisim tr (Tcons st (Tnil (update x (a st) st))).
 
 (* Proposition 3.1: U[x↦e] is setoid. *)
-Definition Updt (u: assertS) (x:id) (a: expr): assertT. 
-exists (updt u x a). 
-move => tr0 [st0 [h0 h1]] tr1 h2. 
-exists st0. foo h1. foo H1. foo h2. foo H2. 
-split; [done | reflexivity]. 
+Definition Updt (u: assertS) (x:id) (a: expr): assertT.
+exists (updt u x a).
+move => tr0 [st0 [h0 h1]] tr1 h2.
+exists st0. inv h1. inv H1. inv h2. inv H2.
+by split=>//; apply: bisim_reflexive.
 Defined.
 
 Definition exS (A: Type) (u: A -> assertS) : assertS :=
@@ -697,310 +715,329 @@ fun st => exists x, u x st.
 
 Definition exT (A: Type) (p: A -> assertT) : assertT.
 exists (fun tr => exists x, satisfy (p x) tr).
-move => tr0 [x h0] tr1 h1. exists x. destruct (p x) as [f0 h2]. 
-simpl. simpl in h0. have := h2 _ h0 _ h1; apply. 
+move => tr0 [x h0] tr1 h1. exists x. destruct (p x) as [f0 h2].
+simpl. simpl in h0. by apply: (h2 _ h0 _ h1).
 Defined.
 
-Definition negT (p: assertT): assertT. 
-destruct p as [f hf]. 
+Definition negT (p: assertT): assertT.
+destruct p as [f hf].
 exists (fun tr => f tr -> False).
-move => tr0 h0 tr1 h1. simpl. move => h2. 
-have := hf _ h2 _ (bisim_symmetric h1). apply h0.
-Defined.      
+move => tr0 h0 tr1 h1 /= h2.
+by move: (hf _ h2 _ (bisim_symmetric h1)).
+Defined.
 
 CoInductive infinite: trace -> Prop :=
 | infinite_delay: forall st tr,
-  infinite tr -> infinite (Tcons st tr). 
+  infinite tr -> infinite (Tcons st tr).
 
 (* Proposition 3.1: Infinite is setoid. *)
 Definition Infinite: assertT.
-exists (fun tr => infinite tr). 
-move => tr0 h0 tr1 h1. simpl. simpl in h0. 
-move: tr0 h0 tr1 h1. cofix hcoind. move => tr0 h0 tr1 h1. 
-foo h0. foo h1. have := infinite_delay st (hcoind _ H _ H3). apply. 
+exists (fun tr => infinite tr).
+move => tr0 /= h0 tr1 h1.
+move: tr0 h0 tr1 h1. cofix hcoind => tr0 h0 tr1 h1.
+inv h0. inv h1. by apply: (infinite_delay st (hcoind _ H _ H3)).
 Defined.
 
 (* Lemma 3.4 (7), => *)
-Lemma infinite_implies_true_chop_false: Infinite =>> (ttT *** [|ffS|]). 
+Lemma infinite_implies_true_chop_false: Infinite =>> (ttT *** [|ffS|]).
 Proof.
-move => tr0 [st0 tr1] hinfinite. simpl. exists (Tcons st0 tr1). split => //. clear tr0.  
-move: st0 tr1 hinfinite. cofix hcofix. 
-* move => st0 tr0 h. apply follows_delay. inversion h. subst. apply hcofix. apply H. 
+move => tr0 [st0 tr1] hinfinite /=. exists (Tcons st0 tr1). split => // {tr0}.
+move: st0 tr1 hinfinite. cofix hcofix.
+move => st0 tr0 h. apply follows_delay. inversion h. subst.
+by apply/hcofix/H.
 Qed.
 
 (* Lemma 3.4 (7), <= *)
-Lemma true_chop_false_implies_infinite: (ttT *** [|ffS|]) =>> Infinite. 
-Proof. 
-move => tr0 [tr1 [_ h1]]. simpl. move: tr0 tr1 h1. cofix h0. move => tr0 tr1 h1. 
-inversion h1; subst; clear h1. 
-- destruct H0 as [st0 [h1 h2]]. inversion h1. 
-- apply infinite_delay. apply (h0 _ _ H). 
-Qed. 
+Lemma true_chop_false_implies_infinite: (ttT *** [|ffS|]) =>> Infinite.
+Proof.
+move => tr0 [tr1 [_ h1]] /=. move: tr0 tr1 h1. cofix h0 => tr0 tr1 h1.
+inv h1.
+- destruct H0 as [st0 [h1 h2]]. by inversion h1.
+- by apply/infinite_delay/(h0 _ _ H).
+Qed.
 
 (* extensions *)
 Lemma iter_split_1: forall p tr, iter p tr -> (singleton ttS tr) \/ (append p (iter p) tr).
-Proof. 
-move => p tr h0. foo h0. 
-- left. exists st. split => //. by apply bisim_reflexive.
-- right. exists tr0. by split. 
-Qed. 
+Proof.
+move => p tr h0. inv h0.
+- left. exists st. split => //. by apply: bisim_reflexive.
+- right. exists tr0. by split.
+Qed.
 
 (* Lemma 3.4 (5), => *)
-Lemma Iter_unfold_0: forall p, Iter p =>> ([|ttS|] orT (p *** Iter p)). 
-Proof. move => [p hp] tr0; simpl => h0. have := iter_split_1 h0. 
-by apply. Qed.
+Lemma Iter_unfold_0: forall p, Iter p =>> ([|ttS|] orT (p *** Iter p)).
+Proof.
+move => [p hp] tr0 /= h0.
+by apply: iter_split_1.
+Qed.
 
-Lemma iter_split_2: forall tr p, (singleton ttS tr) \/ (append p (iter p) tr) -> iter p tr. 
-Proof. 
-move => tr p h. foo h. 
-- move: H => [st [h0 h1]]. foo h1.  apply iter_stop.
-- move: H => [tr0 [h0 h1]]. have := iter_loop h0 h1. by apply. 
-Qed.      
+Lemma iter_split_2: forall tr p, (singleton ttS tr) \/ (append p (iter p) tr) -> iter p tr.
+Proof.
+move => tr p h. inv h.
+- move: H => [st [h0 h1]]. inv h1. by apply: iter_stop.
+- move: H => [tr0 [h0 h1]]. by apply: (iter_loop h0 h1).
+Qed.
 
 (* Lemma 3.4 (5), <= *)
-Lemma Iter_fold_0: forall p, ([|ttS|] orT (p *** Iter p)) =>> Iter p. 
-Proof. move => [p hp] tr0; simpl. apply iter_split_2. Qed.
+Lemma Iter_fold_0: forall p, ([|ttS|] orT (p *** Iter p)) =>> Iter p.
+Proof. move => [p hp] tr0 /=. by apply: iter_split_2. Qed.
 
 Lemma iter_unfold_1: forall p tr, (iter p *+* p) tr -> iter p tr.
-Proof. move => p tr h0.  move: h0 => [tr0 [h0 h1]].
-move: tr0 tr h0 h1. cofix hcoind. move => tr0 tr1 h0 h1. foo h0. 
-- foo h1. have := iter_loop H1. apply. clear H1. move: tr1. cofix hcoind0. 
-  case. move => st. apply follows_nil => //. apply iter_stop. 
-  move => st0 tr0. have := follows_delay _ (hcoind0 _). by apply. 
-- have := iter_loop H. apply. clear H. move: tr tr0 tr1 H0 h1.
-  cofix hcoind0. move => tr0 tr1 tr2 h0 h1. foo h0.
-  - have h0 := follows_hd h1. apply follows_nil => //. 
-    have := hcoind _ _ H0 h1. by apply. 
-  - foo h1. have := follows_delay _ (hcoind0 _ _ _ H H3). by apply. 
-Qed.            
+Proof.
+move => p tr [tr0 [h0 h1]].
+move: tr0 tr h0 h1. cofix hcoind=> tr0 tr1 h0 h1. inv h0.
+- inv h1. apply: (iter_loop H1) => {H1}. move: tr1. cofix hcoind0.
+  case.
+  * move => st. apply: follows_nil => //. by apply: iter_stop.
+  move => st0 tr0. by apply/follows_delay/hcoind0.
+- apply: (iter_loop H) => {H}. move: tr tr0 tr1 H0 h1.
+  cofix hcoind0 => tr0 tr1 tr2 h0 h1. inv h0.
+  - have h0 := follows_hd h1. apply follows_nil => //.
+    by apply: (hcoind _ _ H0 h1).
+  - inv h1. by apply/follows_delay/(hcoind0 _ _ _ H H3).
+Qed.
 
-Lemma Iter_unfold_1: forall p, (Iter p *** p) =>> Iter p. 
-Proof. 
-move => [p hp] tr h0. simpl. simpl in h0.
-have := iter_unfold_1 h0. by apply.
-Qed. 
+Lemma Iter_unfold_1: forall p, (Iter p *** p) =>> Iter p.
+Proof.
+move => [p hp] tr /= h0.
+by apply: iter_unfold_1.
+Qed.
 
-Lemma Iter_unfold_2: forall p, ([|ttS|] orT (Iter p *** p)) =>> Iter p. 
-Proof. move => [p hp] tr0; simpl => h0. foo h0. 
-- destruct H as [st0 [_ h0]]. foo h0. by apply iter_stop. 
-- have := iter_unfold_1 H. by apply. 
-Qed. 
+Lemma Iter_unfold_2: forall p, ([|ttS|] orT (Iter p *** p)) =>> Iter p.
+Proof.
+move=> [p hp] tr0 /= h0. inv h0.
+- move: H => [st0][_]h0. inv h0. by apply: iter_stop.
+by apply: iter_unfold_1.
+Qed.
 
 Lemma Stop_Iter: forall p, [|ttS|] =>> Iter p.
-Proof. move => [p hp]. simpl. move => t0 h0. foo h0. 
-move: H => [_ h0]. foo h0. simpl. apply iter_stop. Qed.   
+Proof.
+move => [p hp] /= t0 h0. inv h0.
+move: H => [_ h0]. inv h0. simpl. by apply: iter_stop.
+Qed.
 
-Lemma Iter_fold_L: forall p, (p *** Iter p) =>> Iter p. 
-Proof. move => [p hp] tr0. simpl. move => [tr1 [h0 h1]]. 
-have := iter_loop h0; apply => //. Qed.
+Lemma Iter_fold_L: forall p, (p *** Iter p) =>> Iter p.
+Proof.
+move => [p hp] tr0 /= [tr1][h0]h1.
+by apply: (iter_loop h0).
+Qed.
 
-Lemma iter_iter_2: forall p tr, iter p tr -> append (iter p) (iter p) tr. 
-Proof. move => p tr0 h0. exists tr0. split => //. clear h0. move: tr0. 
-cofix hcoind. case. 
-- move => st0. apply follows_nil => //. by apply iter_stop. 
-- move => st0 tr0. have := follows_delay _ (hcoind _). by apply. Qed. 
+Lemma iter_iter_2: forall p tr, iter p tr -> append (iter p) (iter p) tr.
+Proof.
+move => p tr0 h0. exists tr0. split => // {h0}. move: tr0.
+cofix hcoind. case=> st0.
+- apply follows_nil => //. by apply iter_stop.
+- move => tr0. by apply/follows_delay/hcoind.
+Qed.
 
-(* Lemma 3.4 (6), => *) 
-Lemma Iter_Iter_2: forall p, Iter p =>> (Iter p *** Iter p). 
-Proof. move => [p hp] tr0. simpl. by apply iter_iter_2. Qed.    
+(* Lemma 3.4 (6), => *)
+Lemma Iter_Iter_2: forall p, Iter p =>> (Iter p *** Iter p).
+Proof. move => [p hp] tr0 /=. by apply: iter_iter_2. Qed.
 
-Lemma iter_iter: forall p tr, append (iter p) (iter p) tr -> (iter p) tr. 
-Proof. move => p tr0 [tr1 [h0 h1]]. move: tr1 tr0 h0 h1. cofix hcoind. 
-move => tr0 tr1 h0. foo h0. 
-- move => h0. foo h0. done. 
-- move => h0. have := iter_loop H. apply. clear H. move: tr tr0 tr1 H0 h0. 
-  cofix hcoind2. move => tr0 tr1 tr2 h0. foo h0. 
-  - move => h0. have h1 := follows_hd h0. apply follows_nil. done. 
-    have := hcoind _ _ H0 h0. done. 
-  - move => h0. foo h0. apply follows_delay.  have := hcoind2 _ _ _ H H3. 
-    done. 
-Qed.                   
+Lemma iter_iter: forall p tr, append (iter p) (iter p) tr -> (iter p) tr.
+Proof. move => p tr0 [tr1 [h0 h1]]. move: tr1 tr0 h0 h1. cofix hcoind.
+move => tr0 tr1 h0. inv h0.
+- move => h0. by inv h0.
+- move => h0. apply: (iter_loop H) => {H}. move: tr tr0 tr1 H0 h0.
+  cofix hcoind2=> tr0 tr1 tr2 h0. inv h0.
+  - move => h0.
+    have h1 := follows_hd h0. apply: follows_nil => //.
+    by apply: (hcoind _ _ H0).
+  - move => h0. inv h0. by apply/follows_delay/(hcoind2 _ _ _ H).
+Qed.
 
 (* Lemma 3.4. (6), <= *)
 Lemma Iter_Iter: forall p, (Iter p *** Iter p) =>> Iter p.
-Proof. move => [p hp]. move => tr. simpl. apply iter_iter. Qed.  
+Proof. move => [p hp] tr /=. by apply: iter_iter. Qed.
 
 (* Lemma 3.1 *)
-Lemma follows_ttS: forall tr, follows (singleton ttS) tr tr. 
-Proof. cofix hcoind. case. 
-- move => st0. apply follows_nil => //. exists st0. split => //. 
-  by apply bisim_reflexive.
-- move => st0 tr0. have := follows_delay _ (hcoind _). apply.  
-Qed.       
+Lemma follows_ttS: forall tr, follows (singleton ttS) tr tr.
+Proof.
+cofix hcoind. case.
+- move => st0. apply follows_nil => //. exists st0. split => //.
+  by apply: bisim_reflexive.
+- move => st0 tr0. by apply/follows_delay/hcoind.
+Qed.
 
 Inductive fin: trace -> state -> Prop :=
 | fin_nil: forall st, fin (Tnil st) st
 | fin_delay: forall st st' tr, fin tr st' -> fin (Tcons st tr) st'.
 
 Lemma append_fin: forall (p q : trace -> Prop) tr0 tr1, p tr0 -> q tr1 -> fin tr0 (hd tr1) ->
-(p *+* q) (tr0 +++ tr1). 
-Proof. move => p q tr0 tr1 hp hq hfin. exists tr0. split => //.
-clear hp. move: tr0 tr1 hq hfin. cofix hcoind. case. 
-- move => st0 tr0 hq h1. rewrite trace_append_nil. foo h1. apply follows_nil => //. 
-- move => st0 tr0 tr1 h0 h1. foo h1. rewrite [Tcons st0 tr0 +++ tr1]trace_destr. 
-  simpl. apply follows_delay. have := hcoind _ _ h0 H2. done.
-Qed.    
+(p *+* q) (tr0 +++ tr1).
+Proof.
+move => p q tr0 tr1 hp hq hfin. exists tr0. split => //.
+clear hp. move: tr0 tr1 hq hfin. cofix hcoind. case.
+- move => st0 tr0 hq h1. rewrite trace_append_nil. inv h1. by apply: follows_nil.
+- move => st0 tr0 tr1 h0 h1. inv h1. rewrite [Tcons st0 tr0 +++ tr1]trace_destr /=.
+  by apply/follows_delay/(hcoind _ _ h0).
+Qed.
 
-Definition last (p: trace -> Prop): assertS := 
+Definition last (p: trace -> Prop): assertS :=
 fun st => exists tr, (p tr) /\ (fin tr st).
 
 Lemma last_cont: forall (p q: trace -> Prop),
 (forall tr, p tr -> q tr) ->
 last p ->> last q.
-Proof. 
-move => p0 p1 hp. move => st [tr [h0 h1]]. 
-exists tr. split. have := hp _ h0; apply. apply h1. 
+Proof.
+move => p0 p1 hp st [tr [h0 h1]].
+exists tr. split=>//. by apply: hp.
 Qed.
 
-Definition Last (p: assertT): assertS. 
-destruct p as  [f0 h0]. apply (last f0).
-Defined.  
+Definition Last (p: assertT): assertS.
+move: p => [f0 h0]. by apply (last f0).
+Defined.
 
 (* Proposition 3.2: Last is monotone. *)
 Lemma Last_monotone: forall p q,
-p =>> q -> Last p ->> Last q. 
-Proof. 
-destruct p as [f hf]. destruct q as [g hg]. simpl. 
-move => h0. apply last_cont. apply h0. 
-Qed. 
+p =>> q -> Last p ->> Last q.
+Proof.
+move=> [f hf] [g hg] /= h0.
+apply/last_cont/h0.
+Qed.
 
 (* Lemma 3.4 (10), => *)
-Lemma Last_Singleton_fold: forall u, Last ([|u|]) ->> u. 
-Proof. 
-move => u st0 h0. destruct h0 as [tr0 [h1 h2]]. destruct h1 as [st1 [h1 h3]]. 
-inversion h3; subst; clear h3. foo h2. exact h1. 
-Qed. 
+Lemma Last_Singleton_fold: forall u, Last ([|u|]) ->> u.
+Proof.
+move => u st0 [tr0] [[st1 [h1 h3]] h2].
+by inv h3; inv h2.
+Qed.
 
 (* Lemma 3.4 (10), <= *)
-Lemma Last_Singleton_unfold: forall u, u ->> Last ([|u|]). 
-Proof. 
+Lemma Last_Singleton_unfold: forall u, u ->> Last ([|u|]).
+Proof.
 move => u st0 h0. exists (Tnil st0). split.
-- exists st0. split; [exact | apply bisim_nil]. 
-- apply fin_nil. 
-Qed. 
+- exists st0. split; [exact | apply bisim_nil].
+- apply: fin_nil.
+Qed.
 
 
 (* Lemma 3.4, (11) *)
 Lemma last_chop: forall p q st, last (append p q) st -> last q st.
-Proof.    
-move => p q st [tr0 [h0 h1]]. move: h0 => [tr [h0 h2]]. clear h0. 
-move: tr0 st h1 tr h2. induction 1. 
-- move => tr0 h0. foo h0. exists (Tnil st). split => //. by apply fin_nil. 
-- move => tr0 h0. foo h0.
-  - exists (Tcons st tr). split => //. have := fin_delay _ h1. by apply.
-  - have := IHh1 _ H1. by apply.
+Proof.
+move => p q st [tr0] [[tr [_ h2]] h1].
+move: tr0 st h1 tr h2. induction 1.
+- move => tr0 h0. inv h0. exists (Tnil st). split => //. by apply fin_nil.
+- move => tr0 h0. inv h0.
+  - exists (Tcons st tr). split => //. by apply: (fin_delay _ h1).
+  - by apply: (IHh1 _ H1).
 Qed.
 
 (* Lemma 3.4, (13) *)
 Lemma Last_chop_sglt: forall p v,
 Last (p *** [|v|]) ->> v.
-Proof. 
-move => [p hp] v. simpl. move => st [tr [[tr' [_ h0]] h1]].
-move: tr st h1 tr' h0. induction 1. 
-- move => tr0 h0. foo h0. move: H0 => [st0 [h0 h1]]. by foo h1.
-- move => tr0 h0. foo h0. 
-  - move: H0 => [st0 [_ h0]]. foo h0. 
-  - have := IHh1 _ H1. by apply.
-Qed. 
+Proof.
+move => [p hp] v /= st [tr [[tr' [_ h0]] h1]].
+move: tr st h1 tr' h0. induction 1.
+- move => tr0 h0. inv h0. move: H0 => [st0 [h0 h1]]. by inv h1.
+- move => tr0 h0. inv h0.
+  - move: H0 => [st0 [_ h0]]. inv h0.
+  - by apply: (IHh1 _ H1).
+Qed.
 
-Lemma Last_andS: forall p u, ((Last p) andS u) ->> Last (p *** [|u|]). 
-Proof. move => p u st0 [h0 h1]. destruct p as [p hp]. simpl in h0. simpl. 
-destruct h0 as [tr0 [h2 h3]]. exists tr0. split => //. exists tr0. split => //. 
-clear h2. move: tr0 st0 h3 h1. cofix hcoind. move => tr0 st0 h0. foo h0. 
-- move => h0. apply follows_nil => //. exists st0. split => //. apply bisim_reflexive. 
-- move => h0. apply follows_delay. have := hcoind _ _ H h0. done.
-Qed.   
+Lemma Last_andS: forall p u, ((Last p) andS u) ->> Last (p *** [|u|]).
+Proof.
+move => [p hp] u st0 [/= [tr0 [h2 h3]] h1].
+exists tr0. split => //. exists tr0. split => // {h2}.
+move: tr0 st0 h3 h1. cofix hcoind. move => tr0 st0 h0. inv h0.
+- move => h0. apply follows_nil => //. exists st0. split => //. apply bisim_reflexive.
+- move => h0. apply follows_delay. apply: (hcoind _ _ H h0).
+Qed.
 
-Lemma iter_last: forall v, 
+Lemma iter_last: forall v,
 ([|v|] *** (Iter (ttT *** Dup v))) =>> (ttT *** [|v|]).
-Proof. 
-move => v. move => tr0 [tr1 [h0 h1]]. move: h0 => [st0 [h0 h2]]. foo h2.
-foo h1. simpl. exists tr0. split => //. move: tr0 h0 H1. cofix hcoind. 
-move => tr0 h0 h1. foo h1. 
+Proof.
+move => v tr0 [tr1 [[st0 [h0 h2]] h1]]. inv h2.
+inv h1. simpl. exists tr0. split => //. move: tr0 h0 H1. cofix hcoind.
+move => tr0 h0 h1. inv h1.
 - apply follows_nil => //. simpl in h0. exists st. split => //.
-  apply bisim_nil. 
+  apply bisim_nil.
 - clear h0. move: H => [tr1 [_ h1]]. move: tr1 tr tr0 h1 H0. cofix hcoind0.
-  move => tr0 tr1 tr2 h0 h1. foo h0. 
-  - move: H0 => [st0 [h0 h2]]. foo h2. foo H1. foo h1. foo H2. 
-    have := follows_delay _ (hcoind _ h0 H1). by apply.   
-  - foo h1. have := follows_delay _ (hcoind0 _ _ _ H H3). apply.
-Qed. 
+  move => tr0 tr1 tr2 h0 h1. inv h0.
+  - move: H0 => [st0 [h0 h2]]. inv h2. inv H1. inv h1. inv H2.
+    by apply/follows_delay/(hcoind _ h0).
+  - inv h1. by apply/follows_delay/(hcoind0 _ _ _ H).
+Qed.
 
 (* Lemma 3.4, (14) *)
 Lemma Last_Sglt_Iter: forall v p,
-Last ([|v|] *** (Iter (p *** Dup v))) ->> v. 
-Proof. move => v p st0 h0.
-have h1: p =>> ttT; first done.  
-have := Last_monotone (Append_monotone_R (Iter_monotone (Append_monotone_L 
-h1))) h0. clear h0 h1. move => h0. 
-have := Last_monotone (@iter_last v) h0 => {h0}. 
-apply Last_chop_sglt.
-Qed.      
+Last ([|v|] *** (Iter (p *** Dup v))) ->> v.
+Proof.
+move => v p st0 h0.
+have h1: p =>> ttT by done.
+have {}h0 := Last_monotone (Append_monotone_R (Iter_monotone (Append_monotone_L
+h1))) h0 => {h1}.
+move: (Last_monotone (@iter_last v) h0) => {h0}.
+by apply: Last_chop_sglt.
+Qed.
 
-Lemma iter_last_dup: forall v, 
+Lemma iter_last_dup: forall v,
 (<<v>> *** (Iter (ttT *** <<v>>))) =>> (ttT *** [|v|]).
-Proof. 
-move => v. move => tr0 [tr1 [h0 h1]]. move: h0 => [st0 [h0 h2]]. foo h2.
-foo H1. foo h1. foo H2. simpl. exists (Tcons (hd tr') tr'). split => //.
-apply follows_delay => //. move: tr' h0 H1. cofix hcoind. 
-move => tr0 h0 h1. foo h1. 
+Proof.
+move=> v tr0 [tr1 [[st0 [h0 h2]] h1]]. inv h2.
+inv H1. inv h1. inv H2. simpl. exists (Tcons (hd tr') tr'). split => //.
+apply follows_delay => //. move: tr' h0 H1. cofix hcoind.
+move => tr0 h0 h1. inv h1.
 - apply follows_nil => //. simpl in h0. exists st. split => //.
-  apply bisim_nil. 
+  apply bisim_nil.
 - clear h0. move: H => [tr1 [_ h1]]. move: tr1 tr tr0 h1 H0. cofix hcoind0.
-  move => tr0 tr1 tr2 h0 h1. foo h0. 
-  - move: H0 => [st0 [h0 h2]]. foo h2. foo H1. foo h1. foo H2. 
-    have := follows_delay _ (hcoind _ h0 H1). by apply.   
-  - foo h1. have := follows_delay _ (hcoind0 _ _ _ H H3). apply.
+  move => tr0 tr1 tr2 h0 h1. inv h0.
+  - move: H0 => [st0 [h0 h2]]. inv h2. inv H1. inv h1. inv H2.
+    by apply/follows_delay/(hcoind _ h0).
+  - inv h1. by apply/follows_delay/(hcoind0 _ _ _ H).
 Qed.
 
 (* Lemma 3.4, (12) *)
-Lemma Last_Last: forall p q, 
-(Last ([| Last p |] *** q)) ->> (Last (p *** q)). 
-Proof. 
-move => p q st0. destruct p as [p hp]. destruct q as [q hq]. 
-simpl. move => [tr1 [h0 h1]]. move: h0 => [tr0 [h0 h2]]. 
-move: h0 => [tr2 [h0 h3]]. foo h3. foo h2. move: h0 => [tr2 [h0 h2]].
-exists (tr2 +++ tr1). split. 
-* exists tr2. split => //. clear h1 h0.
-  move: tr2 h2. cofix hcoind. case. 
-  - move => st1 h0. rewrite trace_append_nil. 
-    apply follows_nil => //. by foo h0. 
-  - move => st1 tr0 h0. foo h0. rewrite trace_append_cons. 
-    apply follows_delay. have := hcoind _ H3. by apply. 
-* clear H1 h0. move h0: (hd tr1) => st1. rewrite h0 in h2. 
-  move: tr2 st1 h2 tr1 h0 h1. induction 1. 
-  - move => tr0 h0 h1. rewrite trace_append_nil. done. 
-  - move => tr0 h0 h1. rewrite trace_append_cons. apply fin_delay. 
-    have := IHh2 _ h0 h1. by apply.
-Qed. 
+Lemma Last_Last: forall p q,
+(Last ([| Last p |] *** q)) ->> (Last (p *** q)).
+Proof.
+move => [p hp] [q hq] st0 /= [tr1 [[tr0 [[tr2 [h0 h3]] h2]] h1]].
+inv h3. inv h2. move: h0 => [tr2 [h0 h2]].
+exists (tr2 +++ tr1). split.
+* exists tr2. split => // {h0 h1}.
+  move: tr2 h2. cofix hcoind. case.
+  - move => st1 h0. rewrite trace_append_nil.
+    apply follows_nil => //. by inv h0.
+  - move => st1 tr0 h0. inv h0. rewrite trace_append_cons.
+    by apply/follows_delay/(hcoind _ H3).
+* clear H1 h0. move h0: (hd tr1) => st1. rewrite h0 in h2.
+  move: tr2 st1 h2 tr1 h0 h1. induction 1.
+  - move => tr0 h0 h1. by rewrite trace_append_nil.
+  - move => tr0 h0 h1. rewrite trace_append_cons.
+    by apply/fin_delay/(IHh2 _ h0 h1).
+Qed.
 
 Lemma singleton_andS_append: forall u v,
-(v andS u) ->> Last ([|v|] *** [|u|]). 
+(v andS u) ->> Last ([|v|] *** [|u|]).
 Proof. move => u v st0 [h0 h1]. exists (Tnil st0). split.
-* exists (Tnil st0). split. exists st0. split => //. apply bisim_reflexive. 
-  apply follows_nil. by simpl. exists st0. split => //. apply bisim_reflexive.  
-* apply fin_nil.
-Qed.  
+* exists (Tnil st0). split.
+  - exists st0. by split => //; apply bisim_reflexive.
+  - apply: follows_nil=>//. exists st0. by split => //; apply: bisim_reflexive.
+* by apply: fin_nil.
+Qed.
 
-Lemma fin_lastdup: forall tr st, fin tr st -> fin (lastdup tr) st. 
+Lemma fin_lastdup: forall tr st, fin tr st -> fin (lastdup tr) st.
 Proof. induction 1.
-- rewrite [lastdup _]trace_destr; simpl. apply fin_delay. apply fin_nil. 
-- rewrite [lastdup _]trace_destr; simpl. apply fin_delay. done.
-Qed.       
+- rewrite [lastdup _]trace_destr /=. by apply/fin_delay/fin_nil.
+- rewrite [lastdup _]trace_destr /=. by apply: fin_delay.
+Qed.
 
-Lemma Last_dup: forall p u, Last (p *** [|u|]) ->> Last (p *** <<u>>). 
-Proof. 
-move => [p hp] u st0 [tr0 [h0 h1]]. move: h0 => [tr1 [h0 h2]].
-exists (lastdup tr0).  split. 
-* have h3 := follows_singleton h2. 
+Lemma Last_dup: forall p u, Last (p *** [|u|]) ->> Last (p *** <<u>>).
+Proof.
+move => [p hp] u st0 [tr0 [[tr1 [h0 h2]] h1]].
+exists (lastdup tr0).  split.
+* have h3 := follows_singleton h2.
   have h4 := follows_setoid (@singleton_setoid _) h2 h3 (bisim_reflexive _) => {h2}.
-  exists tr0. split. have := hp _ h0 _ h3. done. have := follows_dup h4. done.
-* have := fin_lastdup h1. done. 
-Qed. 
+  exists tr0. split.
+  - by apply: (hp _ h0 _ h3).
+  - by apply: (follows_dup h4).
+* by apply: (fin_lastdup h1).
+Qed.
 
 Lemma hd_append: forall tr0 st0, fin tr0 st0 -> forall tr1,
-hd tr1 = st0 -> hd (tr0 +++ tr1) = hd tr0. 
-Proof. induction 1. 
-- move => tr0 h0. rewrite trace_append_nil. done. 
-- move => tr0 h0. rewrite trace_append_cons. by simpl. 
+hd tr1 = st0 -> hd (tr0 +++ tr1) = hd tr0.
+Proof.
+induction 1=> tr0 h0.
+- by rewrite trace_append_nil.
+- by rewrite trace_append_cons.
 Qed.
