theories/AssertClassical.v
@@ -9,12 +9,12 @@ Definition follows_dec : forall p tr0 tr1 (h: follows p tr0 tr1),
  { tr & { st | tr0 = Tnil st /\ hd tr = st /\ p tr } } +
  { tr & { tr' & { st | tr0 = Tcons st tr /\ tr1 = Tcons st tr' /\ follows p tr tr'} } }.
 Proof.
-intros.
+move=>p tr0 tr1 h.
 destruct tr0.
-- left; exists tr1; exists s. by inversion h; subst.
+- left; exists tr1, s. by inversion h; subst.
 - destruct tr1.
-  * left; exists (Tnil s0); exists s0. by inversion h; subst.
-  * right; exists tr0; exists tr1; exists s. by inversion h; subst.
+  * left; exists (Tnil s0), s0. by inversion h; subst.
+  * right; exists tr0, tr1, s. by inversion h; subst.
 Defined.
 
 CoFixpoint midp_dec (p0 p1: trace -> Prop) tr0 tr1 (h: follows (append p0 p1) tr0 tr1) : trace.
@@ -22,10 +22,9 @@ Proof.
 case (follows_dec h).
 - case => tr; case => st; case => h1; case => h2 h3.
   apply constructive_indefinite_description in h3.
-  case: h3 => x [h4 h5].
-  apply x.
+  by case: h3 => x [h4 h5].
 - case => tr; case => tr'; case => st; case => h1; case => h2 h3.
-  apply (Tcons st (@midp_dec _ _ _ _ h3)).
+  by apply (Tcons st (@midp_dec _ _ _ _ h3)).
 Defined.
 
 Lemma midp_midp_dec : forall (p0 p1: trace -> Prop)  tr0 tr1 (h : follows (append p0 p1) tr0 tr1),
@@ -35,31 +34,29 @@ cofix CIH.
 dependent inversion h.
 - subst.
   intros.
-  rewrite [midp_dec _]trace_destr. simpl.
+  rewrite [midp_dec _]trace_destr /=.
   case (constructive_indefinite_description _ _); simpl.
   move => x [a0 hm].
   by apply midp_follows_nil => //; destruct x.
 - subst.
-  rewrite [midp_dec _]trace_destr. simpl.
+  rewrite [midp_dec _]trace_destr /=.
   by apply (@midp_follows_delay p0 p1 (Tcons st tr) (Tcons st tr') (follows_delay st f) tr tr' f st (midp_dec f)).
 Qed.
 
 Lemma append_assoc_R: forall p1 p2 p3,
  forall tr, (append p1 (append p2 p3)) tr -> (append (append p1 p2)  p3) tr.
-Proof. 
-move => p1 p2 p3 tr0 h1.  move: h1 => [tr1 [h1 h2]].
-exists (midp_dec h2). split. 
-- exists tr1. split.
-  * done.  
-  * by have := midp_before (midp_midp_dec h2).
-- by have := midp_after (midp_midp_dec h2).
+Proof.
+move => p1 p2 p3 tr0 [tr1 [h1 h2]].
+exists (midp_dec h2). split.
+- exists tr1. split=>//.
+  by exact: (midp_before (midp_midp_dec h2)).
+- by exact: (midp_after (midp_midp_dec h2)).
 Qed.
 
 (* Lemma 3.4 (4) <= *)
 Lemma Append_assoc_R: forall p1 p2 p3, (p1 *** p2 *** p3) =>> (p1 *** p2) *** p3.
-Proof. 
-move => p1 p2 p3 tr0 h1. destruct p1 as [f1 hf1]. destruct p2 as [f2 hf2]. 
-destruct p3 as [f3 hf3]. simpl. simpl in h1. apply append_assoc_R. by apply h1. 
+Proof.
+move => [f1 hf1] [f2 hf2] [f3 hf3] tr0 /= h1. by apply: append_assoc_R.
 Qed.
 
 Definition Tnil_eq_fin tr st (h : Tnil st = tr) : fin tr st.
@@ -71,7 +68,7 @@ Definition Tcons_eq_fin tr tr' st st' (h : Tcons st tr' = tr) (h': fin tr' st') 
 Proof.
 by rewrite -h; apply fin_delay.
 Defined.
- 
+
 CoFixpoint f (q : trace -> Prop) tr
   (g: forall st, fin tr st -> {tr1 : trace | q tr1 /\ hd tr1 = st}) : trace :=
 match tr as tr' return (tr' = tr -> trace) with
@@ -88,8 +85,7 @@ move => p q tr0 h0 h1 st0 h2.
 have h3: singleton (last p) (Tnil st0).
   by exists st0; split; last apply bisim_reflexive; exists tr0.
 have := h0 _ h3 => {h0 h3} h.
-apply constructive_indefinite_description in h.
-move: h => [tr1 h0]. exists tr1. foo h0. done.
+move/constructive_indefinite_description: h => [tr1 h0]. exists tr1. by inv h0.
 Qed.
 
 Lemma fin_hd_follows : forall q tr0,
@@ -97,12 +93,11 @@ Lemma fin_hd_follows : forall q tr0,
  exists tr1, follows q tr0 tr1.
 Proof.
 move => q tr0 h2. exists (f h2).
-move: tr0 h2. cofix hcoind.
-move => t0. dependent inversion t0.
-- move => h0. rewrite [f _]trace_destr. simpl. 
+move: tr0 h2. cofix hcoind => t0. dependent inversion t0.
+- move => h0. rewrite [f _]trace_destr /=.
   destruct (h0 s (fin_nil s)).
   destruct a.
   by destruct x; apply follows_nil.
-- move => h0. rewrite [f _]trace_destr. simpl. apply follows_delay. 
-  apply hcoind.
+- move => h0. rewrite [f _]trace_destr /=.
+  by apply/follows_delay/hcoind.
 Qed.
