theories/BigFunct.v
@@ -9,68 +9,72 @@ if p st then
   match k st with
   | Tnil st' => Tcons st' (loop k p st')
   | Tcons st' tr => Tcons st' (loopseq k p tr)
-  end 
+  end
 else (Tnil st)
 
 with loopseq (k:state -> trace) (p:state -> bool) (tr:trace) : trace :=
 match tr with
-| Tnil st => Tcons st (loop k p st) 
-| Tcons st tr' => (Tcons st (loopseq k p tr')) 
+| Tnil st => Tcons st (loop k p st)
+| Tcons st tr' => (Tcons st (loopseq k p tr'))
 end.
 
-Lemma loop_true_nil: forall p k st, 
+Lemma loop_true_nil: forall p k st,
 p st = true -> k st = Tnil st -> loop k p st = Tcons st (loop k p st).
 Proof.
-move => p k st h1 h2. rewrite {1}[loop k p st]trace_destr. 
-simpl. rewrite h1. rewrite h2. done. 
-Qed. 
+move => p k st h1 h2.
+by rewrite {1}[loop k p st]trace_destr /= h1 h2.
+Qed.
 
 Lemma loop_true_cons: forall p k st tr,
-p st = true -> k st = Tcons st tr -> loop k p st = Tcons st (loopseq k p tr). 
+p st = true -> k st = Tcons st tr -> loop k p st = Tcons st (loopseq k p tr).
 Proof.
-move => p k st tr h1 h2. rewrite {1}[loop k p st]trace_destr.  
-simpl. rewrite h1. rewrite h2. done. 
-Qed.  
+move => p k st tr h1 h2.
+by rewrite {1}[loop k p st]trace_destr /= h1 h2.
+Qed.
 
 Lemma loop_false: forall k p st, p st = false -> loop k p st = Tnil st.
-Proof. 
-move => k p st h1. rewrite [loop _ _ _]trace_destr. simpl. rewrite h1. done. 
-Qed. 
+Proof.
+move => k p st h1.
+by rewrite [loop _ _ _]trace_destr /= h1.
+Qed.
 
 Lemma loop_nil: forall k p st, loopseq k p (Tnil st) = Tcons st (loop k p st).
 Proof.
-move => k p st. by rewrite {1}[loopseq _ _ _]trace_destr. 
-Qed. 
+move => k p st.
+by rewrite {1}[loopseq _ _ _]trace_destr.
+Qed.
 
-Lemma loopseq_cons: forall k p st tr, 
+Lemma loopseq_cons: forall k p st tr,
 loopseq k p (Tcons st tr) = Tcons st (loopseq k p tr).
 Proof.
-move => k p st tr. by rewrite {1}[loopseq _ _ _]trace_destr. 
-Qed. 
+move => k p st tr.
+by rewrite {1}[loopseq _ _ _]trace_destr.
+Qed.
 
 CoFixpoint sequence (k: state -> trace) (tr:trace): trace :=
 match tr with
 | Tnil st => k st
 | Tcons st tr' => Tcons st (sequence k tr')
-end. 
+end.
 
 Lemma sequence_nil: forall k st, sequence k (Tnil st) = k st.
-Proof. 
-move => k st. rewrite [sequence _ _]trace_destr. 
-simpl. rewrite {2}[k st]trace_destr. rewrite /trace_decompose. done. 
-Qed.    
+Proof.
+move => k st.
+by rewrite [sequence _ _]trace_destr /= {2}[k st]trace_destr /trace_decompose.
+Qed.
 
 Lemma sequence_cons: forall k st tr,
 sequence k (Tcons st tr) = Tcons st (sequence k tr).
-Proof. 
-move => k st tr. rewrite {1}[sequence  _ _]trace_destr. by simpl.  
-Qed.   
+Proof.
+move => k st tr.
+by rewrite {1}[sequence  _ _]trace_destr /=.
+Qed.
 
 Fixpoint Exec (s:stmt) (st: state): trace :=
 match s with
 | Sskip => Tnil st
 | Sassign id a => Tcons st (Tnil (update id (a st) st))
-| Sseq s1 s2 => sequence (Exec s2) (Exec s1 st) 
+| Sseq s1 s2 => sequence (Exec s2) (Exec s1 st)
 | Sifthenelse a s1 s2 =>
   Tcons st (if (is_true (a st)) then (Exec s1 st) else (Exec s2 st))
 | Swhile a s =>
@@ -78,115 +82,113 @@ match s with
 end.
 
 Lemma sequence_correct0: forall s,
-(forall st0, exec s st0 (Exec s st0)) -> 
+(forall st0, exec s st0 (Exec s st0)) ->
 forall tr, execseq s tr (sequence (Exec s) tr).
-Proof. 
-cofix COINDHYP. move => s h1. case. 
+Proof.
+cofix COINDHYP. move => s h1. case.
 - move => st1. apply execseq_nil. rewrite sequence_nil. by apply h1.
-- move => st0 tr0. rewrite sequence_cons. 
-  by apply: (execseq_cons _ (COINDHYP _ h1 _)). 
+- move => st0 tr0. rewrite sequence_cons.
+  by apply: (execseq_cons _ (COINDHYP _ h1 _)).
 Qed.
 
-Lemma Exec_nil: forall s st1 st2, Exec s st1 = Tnil st2 -> st1 = st2. 
-Proof. 
+Lemma Exec_nil: forall s st1 st2, Exec s st1 = Tnil st2 -> st1 = st2.
+Proof.
 move => s; induction s.
-- move => st1 st2 h1. by foo h1.  
-- move => st1 st2 h1. by foo h1.  
-- move => st1 st2 h1. foo h1. case_eq (Exec s1 st1).
-  - move => st3 h2. rewrite h2 in H0. rewrite sequence_nil in H0. 
+- move => st1 st2 h1. by inv h1.
+- move => st1 st2 h1. by inv h1.
+- move => st1 st2 h1. inv h1. case h2: (Exec s1 st1).
+  - rewrite h2 in H0. rewrite sequence_nil in H0.
     move: (IHs1 _ _ h2) => h3 {IHs1 h2}. move: (IHs2 _ _ H0) => h4 {IHs2  H0}.
     by subst.
-  - move => st3 tr1 h2. rewrite h2 in H0. rewrite sequence_cons in H0. by inversion H0. 
-- move => st1 st2 h1. by inversion h1. 
+  - rewrite h2 in H0. rewrite sequence_cons in H0. by inversion H0.
 - move => st1 st2 h1. by inversion h1.
-Qed. 
+- move => st1 st2 h1. by inversion h1.
+Qed.
 
 Lemma sequence_eq_nil: forall s  tr st,
-sequence (Exec s) tr = Tnil st -> tr = Tnil st /\ Exec s st = Tnil st. 
-Proof. 
-move => s. case. 
+sequence (Exec s) tr = Tnil st -> tr = Tnil st /\ Exec s st = Tnil st.
+Proof.
+move => s. case.
 - move => st1 st2 h1. rewrite sequence_nil in h1.
-  move: (Exec_nil h1) => h2. subst. by split.   
-- move => st1 tr st2 h1. rewrite sequence_cons in h1. by inversion h1. 
-Qed. 
+  move: (Exec_nil h1) => h2. subst. by split.
+- move => st1 tr st2 h1. rewrite sequence_cons in h1. by inversion h1.
+Qed.
 
-Lemma Exec_sound_nil: forall s st st', 
+Lemma Exec_sound_nil: forall s st st',
 Exec s st = Tnil st' -> exec s st (Tnil st').
 Proof.
-induction s.  
-- move => st1 st2 h1. simpl in h1. foo h1. by apply exec_skip. 
-- move => st1 st2 h1. simpl in h1. by inversion h1. 
-- move => st1 st2 h1. simpl in h1. move: (sequence_eq_nil h1) => [h2 h3].
+induction s.
+- move => st1 st2 /= h1. inv h1. by apply exec_skip.
+- move => st1 st2 /= h1. by inversion h1.
+- move => st1 st2 /= h1. move: (sequence_eq_nil h1) => [h2 h3].
   move: (IHs1 _ _ h2) => h4 {IHs1 h2}. move: (IHs2 _ _ h3) => h5 {IHs2 h3}.
-  apply: (exec_seq h4). by apply (execseq_nil h5). 
-- move => st1 st2 h1. by inversion h1. 
-- move => st st1 h1. by inversion h1.  
+  apply: (exec_seq h4). by apply (execseq_nil h5).
+- move => st1 st2 h1. by inversion h1.
+- move => st st1 h1. by inversion h1.
 Qed.
 
 Lemma loop_skip_correct: forall s st e,
 Exec s st = Tnil st ->
-is_true (e st) = true ->
+is_true (e st) ->
 exec (Swhile e s) st
- (Tcons st (loop (Exec s) (fun st0 => is_true (e st0)) st)). 
-Proof. 
+ (Tcons st (loop (Exec s) (fun st0 => is_true (e st0)) st)).
+Proof.
 move => s st e h1 h2. cofix COINDHYP.
-apply: (exec_while_loop h2). apply execseq_cons. apply execseq_nil. 
-apply (Exec_sound_nil h1). rewrite [loop _ _ _]trace_destr. simpl.
-rewrite h1. rewrite h2. by apply: (execseq_cons _ (execseq_nil COINDHYP)).  
+apply: (exec_while_loop h2). apply execseq_cons. apply execseq_nil.
+apply (Exec_sound_nil h1). rewrite [loop _ _ _]trace_destr /=.
+rewrite h1 h2. by apply: (execseq_cons _ (execseq_nil COINDHYP)).
 Qed.
 
 Lemma loop_correct0: forall  e s,
 (forall st, exec s st (Exec s st)) ->
 forall st, exec (Swhile e s) st
- (Tcons st (loop (Exec s) (fun st0 => is_true (e st0)) st)). 
+ (Tcons st (loop (Exec s) (fun st0 => is_true (e st0)) st)).
 Proof.
 move => e s h1. cofix COINDHYP.
-have COINDHYP2: forall tr, 
+have COINDHYP2: forall tr,
 execseq  (Swhile e s) tr (loopseq (Exec s) (fun st0 => is_true (e st0)) tr).
-* cofix COINDHYP2. case. 
-  - move => st1. rewrite [loopseq _ _ _]trace_destr; simpl. 
-    by apply: (execseq_nil (COINDHYP _)). 
-  - move => st1 tr1. rewrite [loopseq _ _ _]trace_destr; simpl.  
-    by apply: (execseq_cons _ (COINDHYP2 _)).   
-* move => st. case_eq (is_true (e st)) => h2.
-  - case_eq (Exec s st). 
-    - move => st1 h3. have h4 := (Exec_nil h3). rewrite -h4 in h3. 
-      by apply: (loop_skip_correct h3 h2). 
-    - move => st1 tr1 h3. rewrite [loop _ _ _]trace_destr. simpl.
+* cofix COINDHYP2. case.
+  - move => st1. rewrite [loopseq _ _ _]trace_destr /=.
+    by apply: (execseq_nil (COINDHYP _)).
+  - move => st1 tr1. rewrite [loopseq _ _ _]trace_destr /=.
+    by apply: (execseq_cons _ (COINDHYP2 _)).
+* move => st. case/boolP: (is_true (e st))=>h2.
+  - case h3: (Exec s st).
+    - have h4 := (Exec_nil h3). rewrite -h4 in h3.
+      by apply: (loop_skip_correct h3 h2).
+    - rewrite [loop _ _ _]trace_destr /=.
       rewrite h2. rewrite h3. apply: (exec_while_loop h2 (execseq_cons _  (execseq_nil (h1 _)))).
       rewrite h3.  by apply: (execseq_cons _ (execseq_cons _ (COINDHYP2 _))).
-  - rewrite [loop _ _ _]trace_destr. simpl. rewrite h2. by apply: (exec_while_false _ h2).
-Qed.    
+  - rewrite [loop _ _ _]trace_destr /= (negbTE h2). by apply: (exec_while_false _ h2).
+Qed.
 
 (* the big-step functional semantics correct wrt the big-step relational semantics *)
 Lemma Exec_correct_exec: forall s st, exec s st (Exec s st).
-Proof. 
-move => s; induction s. 
-- move => st. simpl. by apply exec_skip. 
-- move => st. simpl. by apply exec_assign. 
-- move => st. simpl. have h1 := (IHs1 st). 
-  have h2 := sequence_correct0  IHs2 (Exec s1 st). by apply: (exec_seq h1 h2). 
-- move => st. simpl. case_eq (is_true (e st)) => h1. 
+Proof.
+move => s; induction s.
+- move => st /=. by apply exec_skip.
+- move => st /=. by apply exec_assign.
+- move => st /=. have h1 := (IHs1 st).
+  have h2 := sequence_correct0  IHs2 (Exec s1 st). by apply: (exec_seq h1 h2).
+- move => st /=. case/boolP: (is_true (e st))=>h1.
   - apply: (exec_ifthenelse_true _ h1). by apply: (execseq_cons _ (execseq_nil (IHs1 _))).
   - apply: (exec_ifthenelse_false _ h1). by apply: (execseq_cons _ (execseq_nil (IHs2 _))).
-- move => st. simpl. by apply: (loop_correct0 _ IHs).
+- move => st /=. by apply: (loop_correct0 _ IHs).
 Qed.
 
 (* the big-step relational semantics correct wrt the big-step functional semantics *)
 Lemma exec_correct_Exec: forall s st tr, exec s st tr -> bisim tr (Exec s st).
-Proof. 
-move => s st tr h1. have h2 := Exec_correct_exec s st. 
+Proof.
+move => s st tr h1. have h2 := Exec_correct_exec s st.
 by have := exec_deterministic h1 h2; apply.
-Qed.  
+Qed.
 
 Lemma Exec_hd : forall s st, hd (Exec s st) = st.
 Proof.
 elim => //=.
 move => s1 IHs1 s2 IHs2 st.
 case H: (Exec s1 st) => [st'|].
-- apply Exec_nil in H.
-  rewrite -H.
-  by apply IHs2.
-- have IHs1H := IHs1 st.
-  by rewrite H in IHs1H.
+- move/Exec_nil: H=><-.
+  by apply: IHs2.
+- by move: (IHs1 st); rewrite H.
 Qed.
