theories/Hoare.v
@@ -9,10 +9,10 @@ fun st => exists st0 : state, (u st0) /\ (update x (a st0) st0 = st).
 
 Inductive hsemax : assertS -> stmt -> assertS -> Prop :=
 
-| hsemax_skip: forall u,   hsemax u Sskip u 
+| hsemax_skip: forall u,   hsemax u Sskip u
 
-| hsemax_assign: forall u x a, 
-  hsemax u (Sassign x a) (udt u x a) 
+| hsemax_assign: forall u x a,
+  hsemax u (Sassign x a) (udt u x a)
 
 | hsemax_seq: forall s1 s2 u1 u2 u3,
   hsemax u1 s1 u2->
@@ -25,18 +25,18 @@ Inductive hsemax : assertS -> stmt -> assertS -> Prop :=
   hsemax u1 (Sifthenelse a s1 s2) u2
 
 | hsemax_while:forall a s u,
-  hsemax  (u andS eval_true a) s u ->
+  hsemax (u andS eval_true a) s u ->
   hsemax u (Swhile a s) (u andS eval_false a)
 
 | hsemax_conseq: forall s u1 u2 v1 v2,
-  u1 ->> u2 -> 
-  v2 ->> v1 -> 
+  u1 ->> u2 ->
+  v2 ->> v1 ->
   hsemax u2 s v2 ->
   hsemax u1 s v1
 
 | hsemax_ex: forall s (A : Type) (u: A -> assertS) (v: A -> assertS),
   (forall x, hsemax (u x) s (v x)) ->
-  hsemax (exS u) s (exS v). 
+  hsemax (exS u) s (exS v).
 
 Lemma hsemax_conseq_L: forall s u1 u2 v,
 u1 ->> u2 -> hsemax u2 s v -> hsemax u1 s v.
@@ -46,216 +46,220 @@ exact: hsemax_conseq h0 (@assertS_imp_refl v) h1.
 Qed.
 
 Lemma hsemax_conseq_R: forall s u v1 v2,
-v2 ->> v1 -> hsemax u s v2 -> hsemax u s v1. 
-Proof. 
-move => s u v1 v2 h0 h1. 
-have := hsemax_conseq (@assertS_imp_refl u)  h0 h1. 
-by apply. 
+v2 ->> v1 -> hsemax u s v2 -> hsemax u s v1.
+Proof.
+move => s u v1 v2 h0 h1.
+have := hsemax_conseq (@assertS_imp_refl u)  h0 h1.
+by apply.
 Qed.
 
 Lemma Last_destruct : forall (p: assertT) st tr,
  satisfy p tr -> fin tr st -> Last p st.
-Proof. 
-move => [f h] st tr h0 h1. simpl. simpl in h0. exists tr. 
-by split. 
+Proof.
+move => [f h] st tr /= h0 h1. exists tr.
+by split.
 Qed.
 
-(* Proposition 4.3: projecting the trace-based Hoare logic into 
+(* Proposition 4.3: projecting the trace-based Hoare logic into
    the partial-correctness Hoare logic. *)
-Lemma semax_correct_hsemax: forall u s p, 
+Lemma semax_correct_hsemax: forall u s p,
 semax u s p -> forall v, hsemax (v andS u) s (Last ([|v|] *** p)).
 Proof.
-induction 1. 
+induction 1.
 - move => v. have h0 := hsemax_skip (v andS u).
   have h1 := (@singleton_andS_append u v).
-  have := hsemax_conseq_R h1 h0. by apply.  
+  by apply: (hsemax_conseq_R h1 h0).
 - move => v. have h0 := hsemax_assign (v andS u) x a.
-  have h1: (udt (v andS u) x a) ->> (Last ([|v|] *** Updt u x a)). 
-  * clear h0. move => st0 h0. move: h0 => [st1 [[h0 h1] h2]]. 
-     exists (Tcons st1 (Tnil st0)). split. exists (Tnil st1). split. 
-     exists st1; split => //. by apply bisim_reflexive. apply follows_nil.
-     by simpl. rewrite /updt. exists st1. split => //.
-     rewrite h2. by apply bisim_reflexive. apply fin_delay. apply fin_nil.  
-  have := hsemax_conseq_R h1 h0. by apply. 
-- move => v0. 
-  have h: Last ([|Last ([|v0|] *** p1 *** [|v|])|] *** p2) ->> 
+  have h1: (udt (v andS u) x a) ->> (Last ([|v|] *** Updt u x a)).
+  * move => st0 [st1 [[{}h0 h1] h2]].
+    exists (Tcons st1 (Tnil st0)). split.
+    + exists (Tnil st1). split.
+      - exists st1; split => //. by apply bisim_reflexive.
+      apply: follows_nil=>//. rewrite /updt. exists st1. split => //.
+      rewrite h2. by apply: bisim_reflexive.
+    by apply/fin_delay/fin_nil.
+  by apply: (hsemax_conseq_R h1 h0).
+- move => v0.
+  have h: Last ([|Last ([|v0|] *** p1 *** [|v|])|] *** p2) ->>
   Last ([|v0|] *** p1 *** p2).
   * move => st0 h0. have h1 := Last_Last h0 => {h0}.
-    have := Last_monotone _ h1 => {h1}. apply. clear st0. 
-    have h0 := (@Append_assoc_L ([|v0|]) (p1 *** ([|v|])) p2). 
-    have := impT_conseq_L h0. apply. clear h0.
-    apply Append_monotone_R. apply Append_monotone_L. apply Append_Singleton. 
-  have := hsemax_conseq_R h. apply. have := hsemax_seq (IHsemax1 _). apply. 
-  have := hsemax_conseq_L _ (IHsemax2 _). apply. move => st0. move => h0. 
-  split. done. have := (@Last_chop_sglt ([|v0|] *** p1) v). apply. 
-  have := Last_monotone _ h0. apply. apply Append_assoc_R.   
+    apply: (Last_monotone _ h1) => {h1 st0}.
+    have h0 := (@Append_assoc_L ([|v0|]) (p1 *** ([|v|])) p2).
+    apply: (impT_conseq_L h0) => {h0}.
+    by apply/Append_monotone_R/Append_monotone_L/Append_Singleton.
+  apply/(hsemax_conseq_R h)/(hsemax_seq (IHsemax1 _))/(hsemax_conseq_L _ (IHsemax2 _)).
+  move => st0 h0. split=>//.
+  by apply/(@Last_chop_sglt ([|v0|] *** p1) v)/(Last_monotone _ h0)/Append_assoc_R.
 - move => v.
-  have hpost : (Last ([|v andS u|] *** p)) ->> (Last ([|v|] *** <<u>> *** p)). 
-  * destruct p as [p hp]. move => st0 h0. simpl. move: h0 => [tr0 [h0 h1]]. 
-     move: h0 => [tr1 [h0 h2]]. move: h0 => [st1 [h4 h3]]. foo h3. 
-     foo h2. move: h4 => [h2 h3]. exists (Tcons (hd tr0) tr0). 
-     split. exists (Tnil (hd tr0)). split. exists (hd tr0). 
-     split => //. by apply bisim_reflexive. apply follows_nil =>//.
-     exists (Tcons (hd tr0) (Tnil (hd tr0))). split. exists (hd tr0). 
-     split => //. by apply bisim_reflexive. apply follows_delay.
-     apply follows_nil =>//. apply fin_delay. done. 
-  apply hsemax_ifthenelse. 
-  * have hpre: ((v andS u) andS eval_true a) ->> 
+  have hpost : (Last ([|v andS u|] *** p)) ->> (Last ([|v|] *** <<u>> *** p)).
+  * destruct p as [p hp]. move => st0 [tr0 [[tr1 [[st1 [h4 h3]] h2]] h1]] /=.
+     inv h3. inv h2. move: h4 => [h2 h3]. exists (Tcons (hd tr0) tr0).
+     split.
+     + exists (Tnil (hd tr0)). split.
+       - exists (hd tr0). split => //. by apply bisim_reflexive.
+       apply follows_nil =>//.
+       exists (Tcons (hd tr0) (Tnil (hd tr0))). split.
+       - exists (hd tr0). split => //. by apply bisim_reflexive.
+       apply/follows_delay/follows_nil =>//. by apply: fin_delay.
+  apply hsemax_ifthenelse.
+  * have hpre: ((v andS u) andS eval_true a) ->>
      ((v andS u) andS u andS eval_true a).
-      * move => st0 [h0 h1]. split => //. move: h0 => [h0 h2]. by split. 
+      * move => st0 [h0 h1]. split => //. move: h0 => [h0 h2]. by split.
      have h0 := IHsemax1 (v andS u) => {IHsemax1}.
-     have := hsemax_conseq_L hpre h0 => {h0}. move => h0. 
-     have := hsemax_conseq_R hpost h0. apply.
-  * have hpre: ((v andS u) andS eval_false a) ->> 
+     move: (hsemax_conseq_L hpre h0) => {}h0.
+     apply: (hsemax_conseq_R hpost h0).
+  * have hpre: ((v andS u) andS eval_false a) ->>
      ((v andS u) andS u andS eval_false a).
-      * move => st0 [h0 h1]. split => //. move: h0 => [h0 h2]. by split.  
-     have h0 := IHsemax2 (v andS u) => {IHsemax1 IHsemax2}. 
-     have := hsemax_conseq_L hpre h0 => {h0}. move => h0. 
-     have := hsemax_conseq_R hpost h0. apply. 
-- move => w.  
-  set inv := Last ([|w|] *** <<u0>> *** Iter ( p *** <<u>>)). 
+      * move => st0 [h0 h1]. split => //. move: h0 => [h0 h2]. by split.
+     have h0 := IHsemax2 (v andS u) => {IHsemax1 IHsemax2}.
+     move: (hsemax_conseq_L hpre h0) => {}h0.
+     apply: (hsemax_conseq_R hpost h0).
+- move => w.
+  set inv := Last ([|w|] *** <<u0>> *** Iter ( p *** <<u>>)).
   have h0 := IHsemax inv => {IHsemax H0}.
   have h1: (inv andS eval_true a) ->> (inv andS u andS eval_true a).
-  * clear h0. move => st [h0 h1]. split => //. split => //. clear h1. 
-    destruct p as [f hf]. simpl in inv. move: h0 => [tr [h0 h1]]. 
-    move: h0 => [tr0 [h0 h2]]. move: h0 => [st0 [_ h3]]. foo h3.
-    foo h2. move: H2 => [tr0 [h3 h2]]. move: h3 => [st0 [h3 h4]]. foo h4. 
-    foo H2. foo h2. foo h1. foo H3. have h0 := H _ h3 => {h3}.
-    have h1: satisfy (ttT *** [|u|]) tr'. 
-    * apply iter_last. simpl. exists (Tnil (hd tr')). split. 
-      exists (hd tr'). split => //. by apply bisim_nil. 
-      apply follows_nil => //. 
-      have := iter_cont (@append_cont_L _ _ _ _)  H2.
-      apply. done. 
-    simpl in h1. clear H2 h0. move: h1 => [tr0 [_ h1]]. 
-    move: tr' st H4 tr0 h1. induction 1. 
-    - move => tr0 h0. foo h0. move: H1 => [st0 [h0 h1]]. by foo h1.
-    - move => tr0 h0. foo h0. move: H1 => [st0 [_ h0]]. foo h0. 
-      have := IHfin _ H2. by apply.            
+  * move => st [{}h0 h1]. do!split => //. clear h1.
+    destruct p as [f hf]. simpl in inv.
+    move: h0 => [tr [[tr0 [[st0 [_ h3]] h2]] h1]].
+    inv h3. inv h2. move: H2 => [tr0 [[st0 [h3 h4]] h2]]. inv h4.
+    inv H2. inv h2. inv h1. inv H3. have h0 := H _ h3 => {h3}.
+    have h1: satisfy (ttT *** [|u|]) tr'.
+    * apply iter_last. simpl. exists (Tnil (hd tr')). split.
+      exists (hd tr'). split => //. by apply bisim_nil.
+      apply follows_nil => //.
+      by apply: (iter_cont (@append_cont_L _ _ _ _) H2).
+    simpl in h1. clear H2 h0. move: h1 => [tr0 [_ h1]].
+    move: tr' st H4 tr0 h1. induction 1.
+    - move => tr0 h0. inv h0. move: H1 => [st0 [h0 h1]]. by inv h1.
+    - move => tr0 h0. inv h0. move: H1 => [st0 [_ h0]]. inv h0.
+      by apply: (IHfin _ H2).
   have h2 := hsemax_conseq_L h1 h0 => {h0 h1}.
   have h0 : Last ([|inv|] *** p *** [|u|]) ->> inv.
-  * clear h2.  move => st0 h0. have h1 := Last_Last h0 => {h0}.
-    have := Last_monotone (@Append_assoc_L _ _ _). apply.  
-    have := Last_monotone (@Append_monotone_R _ _ _ (@Iter_unfold_1 _)). 
-    apply. have := Last_monotone (@Append_assoc_L _ _ _). apply. 
-    have := Last_monotone (@Append_assoc_L _ _ _). apply. 
+  * move => {h2} st0 h0. have h1 := Last_Last h0 => {h0}.
+    apply: (Last_monotone (@Append_assoc_L _ _ _)).
+    apply: (Last_monotone (@Append_monotone_R _ _ _ (@Iter_unfold_1 _))).
+    apply: (Last_monotone (@Append_assoc_L _ _ _)).
+    apply: (Last_monotone (@Append_assoc_L _ _ _)).
     have : Last ((((([|w|]) *** (<< u0 >>)) *** Iter (p *** (<< u >>))) *** p) ***
     ([|u|])) st0.
-    * have := Last_monotone (@Append_assoc_R _ _ _). apply.
-       have := Last_monotone (Append_monotone_L (@Append_assoc_R _ _ _)).
-       apply. done. clear h1. move => h1.  
-       have := Last_dup h1. done. 
-    have h1 := hsemax_conseq_R h0 h2 => {h0 h2}.
-    have h0 := hsemax_while h1 => {h1}. 
-    have := hsemax_conseq _ _ h0. apply. 
-    * clear h0. move => st0 h0. rewrite /inv. have := Last_monotone 
-      (@Append_monotone_R _ _ _ (@Append_monotone_R  _ _ _ (@Stop_Iter _))).
-      apply. move: h0 => [h0 h1].  exists (Tcons st0 (Tnil st0)). split.
-      exists (Tnil st0). split. exists st0. split => //. apply bisim_reflexive. 
-      apply follows_nil. by simpl. exists (Tcons st0 (Tnil st0)). split. 
-      exists st0. split => //. by apply bisim_reflexive. apply follows_delay. 
-      apply follows_nil. by simpl. exists st0. split => //. by apply bisim_reflexive. 
-      apply fin_delay. apply fin_nil. 
-    * rewrite /inv. move => st0 [h1 h2]. 
-      have := Last_monotone (@Append_assoc_L _ _ _). apply. 
-      have := Last_monotone (@Append_assoc_L _ _ _). apply.
-      have := Last_monotone (@Append_monotone_L _ _ _ (@Append_assoc_R _ _ _)). 
-      apply. destruct p as [p hp]. move: h1 => [tr0 [h1 h3]]. simpl.
-      exists tr0. split => //. exists tr0. split => //. clear h1. move: tr0 h3.
-      cofix hcoind. move => tr0 h1. foo h1. apply follows_nil. by simpl.
-      exists st0. split => //. apply bisim_reflexive. apply follows_delay. 
-      have := hcoind _ H0. by apply.         
-- move => v. have h := IHsemax v => {IHsemax}. 
+    * apply: (Last_monotone (@Append_assoc_R _ _ _)).
+      by apply: (Last_monotone (Append_monotone_L (@Append_assoc_R _ _ _))).
+    by apply/Last_dup.
+  have h1 := hsemax_conseq_R h0 h2 => {h0 h2}.
+  have h0 := hsemax_while h1 => {h1}.
+  apply: (hsemax_conseq _ _ h0).
+  * move => st0 {}h0. rewrite /inv.
+    apply: (Last_monotone
+    (@Append_monotone_R _ _ _ (@Append_monotone_R  _ _ _ (@Stop_Iter _)))).
+    move: h0 => [h0 h1]. exists (Tcons st0 (Tnil st0)). split.
+    + exists (Tnil st0). split.
+      - exists st0. split => //. by apply: bisim_reflexive.
+      apply: follows_nil=>//. exists (Tcons st0 (Tnil st0)). split.
+      - exists st0. split => //. by apply bisim_reflexive.
+      apply/follows_delay/follows_nil=>//. exists st0. split => //. by apply bisim_reflexive.
+    by apply/fin_delay/fin_nil.
+  * rewrite /inv => st0 [h1 h2].
+    apply: (Last_monotone (@Append_assoc_L _ _ _)).
+    apply: (Last_monotone (@Append_assoc_L _ _ _)).
+    apply: (Last_monotone (@Append_monotone_L _ _ _ (@Append_assoc_R _ _ _))).
+    destruct p as [p hp]. move: h1 => [tr0 [h1 h3]] /=.
+    exists tr0. split => //. exists tr0. split => // {h1}. move: tr0 h3.
+    cofix hcoind. move => tr0 h1. inv h1.
+    + apply follows_nil=>//. exists st0. split => //. by apply: bisim_reflexive.
+    by apply/follows_delay/hcoind.
+- move => v. have h := IHsemax v => {IHsemax}.
   have h0 := andS_cont (@assertS_imp_refl _) H.
-  have := hsemax_conseq_L (h0 _). apply. clear h0. 
-  have := hsemax_conseq_R _ h. apply. clear h. 
-  apply Last_monotone. have := Append_monotone_R. apply. done. 
-- move => v.    
-  have: (v andS exS u) ->> (exS (fun a => v andS u a)).
-  * move => st0 [h0 [x h1]]. exists x. split => //. 
-  move => h0. have := hsemax_conseq_L h0 => {h0}. apply.   
-  have: (exS (fun x => Last ([|v|] *** (p x)))) ->> Last ([|v|] *** exT p).
-  * move => st0. move => [x h0]. move hp: (p x) => q. rewrite hp in h0. 
+  apply: (hsemax_conseq_L (h0 _)) => {h0}.
+  apply: (hsemax_conseq_R _ h) => {h}.
+  by apply/Last_monotone/Append_monotone_R.
+- move => v.
+  have h0: (v andS exS u) ->> (exS (fun a => v andS u a)).
+  * move => st0 [h0 [x h1]]. exists x. by split.
+  apply: (hsemax_conseq_L h0) => {h0}.
+  have h0: (exS (fun x => Last ([|v|] *** (p x)))) ->> Last ([|v|] *** exT p).
+  * move => st0 [x h0]. move hp: (p x) => q. rewrite hp in h0.
     destruct q as [q hq]. simpl in h0. destruct h0 as [tr0 [h0 h1]].
-    exists tr0. split => //. clear h1. destruct h0 as [tr1 [h0 h1]]. 
+    exists tr0. split => //. clear h1. destruct h0 as [tr1 [h0 h1]].
     exists tr1. split => //. clear h0. move: tr1 tr0 h1. cofix hcoind.
-    move => tr0 tr1 h0. foo h0. apply follows_nil => //. exists x.
+    move => tr0 tr1 h0. inv h0. apply follows_nil => //. exists x.
     rewrite hp. simpl => //. apply follows_delay.
-    have := hcoind _ _ H1. done. 
-  move => h0. have := hsemax_conseq_R h0. apply. clear h0. 
-  apply hsemax_ex. done. 
+    by apply: hcoind.
+  apply: (hsemax_conseq_R h0)=>{h0}.
+  by apply: hsemax_ex.
 Qed.
 
 (* Corollary 4.2 *)
-Lemma semax_correct_hsemax_main: forall u s p, 
+Lemma semax_correct_hsemax_main: forall u s p,
 semax u s p -> hsemax u s (Last p).
 Proof.
-move => U s P hhsemax. have := (semax_correct_hsemax hhsemax ttS) => {hhsemax}.
-move => hhsemax. have := (hsemax_conseq _ _ hhsemax); apply => {hhsemax}. 
- * move => st0 hU. split => //. 
+move => U s P hhsemax.
+move: (semax_correct_hsemax hhsemax ttS) => {}hhsemax.
+apply: (hsemax_conseq _ _ hhsemax) => {hhsemax}.
+ * move => st0 hU. by split.
  * move => st0 h0. destruct P as [P hP]. destruct h0 as [tr0 [h0 h1]].
-   exists tr0. split => //. destruct h0 as [h0  [h2 h3]]. 
-   inversion h2; subst; clear h2. destruct H as [_ h2]. clear h1. 
-   inversion h2; subst; clear h2. inversion h3; subst; clear h3. 
-   done. 
-Qed. 
+   exists tr0. split => //. destruct h0 as [h0  [h2 h3]].
+   inversion h2; subst; clear h2. destruct H as [_ h2]. clear h1.
+   inversion h2; subst; clear h2. inversion h3; by subst.
+Qed.
 
-(* Proposition 4.1: embedding the partial-correctness Hoare logic 
+(* Proposition 4.1: embedding the partial-correctness Hoare logic
    into the trace-based Hoare logic *)
-Lemma hsemax_correct_semax: forall u s v, 
-hsemax u s v -> semax u s (ttT *** [|v|]). 
-Proof. 
+Lemma hsemax_correct_semax: forall u s v,
+hsemax u s v -> semax u s (ttT *** [|v|]).
+Proof.
 induction 1.
 - have h0 := semax_skip u.
   have h1: ([|u|]) =>> (ttT *** [|u|]).
-  * move => tr0 [st0 [h1 h2]]. foo h2. exists (Tnil st0). split => //. 
-     apply follows_nil =>//. exists st0. split; [done | apply bisim_nil]. 
-  have := semax_conseq_R h1 h0. by apply.     
-- have h0 := semax_assign u x a. 
-  have h1: (Updt u x a) =>> (ttT *** [|udt u x a|]). 
-  * move => tr0 [st0 [h1 h2]]. exists tr0. split => //. foo h2. foo H1.
-    apply follows_delay. apply follows_nil. by simpl. exists (update x (a st0) st0). 
-    split; last apply bisim_nil. exists st0. by split.   
-  have := semax_conseq_R h1 h0. by apply.  
-- have h0 := semax_seq IHhsemax1 IHhsemax2 => {IHhsemax1 IHhsemax2}. 
+  * move => tr0 [st0 [h1 h2]]. inv h2. exists (Tnil st0). split => //.
+     apply follows_nil =>//. exists st0. split; [done | apply bisim_nil].
+  by apply: (semax_conseq_R h1 h0).
+- have h0 := semax_assign u x a.
+  have h1: (Updt u x a) =>> (ttT *** [|udt u x a|]).
+  * move => tr0 [st0 [h1 h2]]. exists tr0. split => //. inv h2. inv H1.
+    apply/follows_delay/follows_nil=>//.
+    exists (update x (a st0) st0).
+    split; last by apply bisim_nil. exists st0. by split.
+  by apply: (semax_conseq_R h1 h0).
+- have h0 := semax_seq IHhsemax1 IHhsemax2 => {IHhsemax1 IHhsemax2}.
   have h1 := semax_conseq_R (@Append_assoc_R _ _ _) h0 => {h0}.
-  have := (semax_conseq_R (@Append_monotone_L _ _ _ (@ttT_idem_comp)) h1).
-  by apply. 
-- have h0 := semax_ifthenelse IHhsemax1 IHhsemax2 => {IHhsemax1 IHhsemax2 H H0}. 
-  have h1: (<<u1>> *** ttT *** [|u2|]) =>> (ttT *** [|u2|]). 
-  * clear h0. move => tr0 h0. have h1 := append_assoc_R h0 => {h0}.
-    move: h1 => [tr1 [h0 h1]]. exists tr1. by split. 
-  have := semax_conseq_R h1 h0. by apply.      
-- have h0: u ->> u; first done.
-  have h1 := semax_while h0 IHhsemax => {h0 IHhsemax}.  
+  apply: (semax_conseq_R (@Append_monotone_L _ _ _ (@ttT_idem_comp)) h1).
+- have h0 := semax_ifthenelse IHhsemax1 IHhsemax2 => {IHhsemax1 IHhsemax2 H H0}.
+  have h1: (<<u1>> *** ttT *** [|u2|]) =>> (ttT *** [|u2|]).
+  * move => tr0 {}h0. move: (append_assoc_R h0) => [tr1 [{}h0 h1]].
+    exists tr1. by split.
+  by apply: (semax_conseq_R h1 h0).
+- have h0: u ->> u by [].
+  have h1 := semax_while h0 IHhsemax => {h0 IHhsemax}.
   set p0 := (ttT *** << u >>).
-  have h0: ((<< u >>) *** Iter p0 *** [|eval_false a|]) =>> 
-  (ttT *** [|u andS eval_false a|]). 
-  * clear h1. move => tr0 [tr1 [h0 h1]]. move: h0 => [st0 [h0 h2]].
-     foo h2. foo H2. foo h1. foo H3. exists (Tcons (hd tr') tr'). 
-     split; first done. apply follows_delay. move: tr' H2 h0. 
-     cofix hcoind0. move => tr0 h0 h1. move: h0 => [tr1 [h0 h2]].
-     foo h0. foo h2. move: H2 => [st0 [h0 h2]]. foo h2. simpl in h1. 
-     apply follows_nil => //. exists st0. split => //. apply bisim_reflexive.
-     clear h1. move: tr tr1 tr0 H0 H1 h2. cofix hcoind1. 
-     move => tr0 tr1 tr2 h0 h1 h2. move: h0 => [tr3 [h0 h3]]. foo h3. 
-     clear h0. move: H1 => [st0 [h0 h3]]. foo h3. foo H2. foo h1. 
-    foo H3. foo h2. have h1 := follows_hd H4. rewrite h1 in h0 => {h1}. 
-    have := follows_delay (hd tr'). apply. have := hcoind0 _ _ h0. apply.
-    exists tr'. split; by [apply H4 | apply H2]. foo h1. foo h2. 
-    clear h0 hcoind0. apply follows_delay. 
-    have := hcoind1 _ _ _ _ H4 H5. apply. exists tr. split; [done | apply H0].  
-  have := semax_conseq_R h0 h1. by apply.   
+  have h0: ((<< u >>) *** Iter p0 *** [|eval_false a|]) =>>
+  (ttT *** [|u andS eval_false a|]).
+  * move => tr0 [tr1 [[st0 [h0 h2]] {}h1]].
+    inv h2. inv H2. inv h1. inv H3. exists (Tcons (hd tr') tr').
+    split=>//. apply follows_delay. move: tr' H2 h0.
+    cofix hcoind0. move => tr0 [tr1 [h0 h2]] h1.
+    inv h0. inv h2. move: H2 => [st0 [h0 h2]]. inv h2. simpl in h1.
+    apply follows_nil => //. exists st0. split => //. by apply: bisim_reflexive.
+    clear h1. move: tr tr1 tr0 H0 H1 h2. cofix hcoind1.
+    move => tr0 tr1 tr2 [tr3 [h0 h3]] h1 h2. inv h3.
+    + clear h0. move: H1 => [st0 [h0 h3]]. inv h3. inv H2. inv h1.
+      inv H3. inv h2. rewrite (follows_hd H4) in h0.
+      apply: (follows_delay (hd tr')); apply: (hcoind0 _ _ h0).
+      exists tr'. split; by [apply H4 | apply H2].
+    inv h1. inv h2.
+    clear h0 hcoind0. apply follows_delay.
+    apply: (hcoind1 _ _ _ _ H4 H5). exists tr. by split=>//; apply H0.
+  by apply: (semax_conseq_R h0 h1).
 - have h0 := Singleton_monotone H0.
   have h1 := (@Append_monotone_R ttT _ _ h0) => {h0}.
   have h0 := semax_conseq_R h1 IHhsemax => {h1 IHhsemax}.
-  have := semax_conseq_L H h0. apply. 
-- have: (exT (fun x => ttT *** [|v x|])) =>> (ttT *** [|exS v|]). 
-  * move => tr0 [x h0]. simpl in h0. simpl. destruct h0 as [tr1 [h0 h1]]. 
-    exists tr1. split => //. clear h0. move: tr1 tr0 h1. cofix hcoind. 
-    move => tr0 tr1 h0. foo h0. apply follows_nil => //. destruct H2 as [st0 [h0 h1]]. 
-    exists st0; split => //. exists x. done. apply follows_delay. 
-    have := hcoind _ _ H1. apply. 
-  move => h0. have := semax_conseq_R h0. apply. clear h0. 
-  apply semax_ex =>//.   
+  apply: (semax_conseq_L H h0).
+- have h0: (exT (fun x => ttT *** [|v x|])) =>> (ttT *** [|exS v|]).
+  * move => tr0 [x h0]. simpl in h0. simpl. destruct h0 as [tr1 [h0 h1]].
+    exists tr1. split => //. clear h0. move: tr1 tr0 h1. cofix hcoind.
+    move => tr0 tr1 h0. inv h0.
+    + apply follows_nil => //. destruct H2 as [st0 [h0 h1]].
+      exists st0; split => //. by exists x.
+    by apply/follows_delay/hcoind.
+  apply: (semax_conseq_R h0) => {h0}.
+  by apply semax_ex.
 Qed.
