theories/Liveness.v
@@ -7,7 +7,7 @@ Import Prenex Implicits.
 
 Variable x : id.
 Variable tt : expr.
-Axiom tt_true : forall st, is_true (tt st) = true.
+Axiom tt_true : forall st, is_true (tt st).
 
 Definition incr_x : expr := fun st => st x + 1.
 Definition x_is_zero : assertS := fun st => st x = 0.
@@ -19,22 +19,22 @@ Proof. by rewrite /update Nat.eqb_refl. Qed.
 Inductive eventually_x_is_n (n: nat) : trace -> Prop :=
 | x_is_n_nil: forall st, st x = n -> eventually_x_is_n n (Tnil st)
 | x_is_n_cons: forall st tr, st x = n -> eventually_x_is_n n (Tcons st tr)
-| x_is_n_delay: forall st tr, 
+| x_is_n_delay: forall st tr,
   eventually_x_is_n n tr -> eventually_x_is_n n (Tcons st tr).
 
 Lemma eventually_x_is_n_setoid: forall n tr,
  eventually_x_is_n n tr -> forall tr0, bisim tr tr0 ->
  eventually_x_is_n n tr0.
-Proof. 
-induction 1. 
-- move => tr0 h0. foo h0. apply x_is_n_nil => //. 
-- move => tr0 h0. foo h0. apply x_is_n_cons => //.
-- move => tr0 h0. foo h0. apply x_is_n_delay. 
-  have := IHeventually_x_is_n _ H3. done. 
+Proof.
+induction 1.
+- move => tr0 h0. inv h0. apply x_is_n_nil => //.
+- move => tr0 h0. inv h0. apply x_is_n_cons => //.
+- move => tr0 h0. inv h0. apply x_is_n_delay.
+  exact: (IHeventually_x_is_n _ H3).
 Qed.
 
-Definition Eventually_x_is_n (n:nat): assertT. 
-exists (eventually_x_is_n n). 
+Definition Eventually_x_is_n (n:nat): assertT.
+exists (eventually_x_is_n n).
 move => tr0 h0 tr1 h1. exact: (eventually_x_is_n_setoid h0 h1).
 Defined.
 
@@ -45,62 +45,63 @@ Definition s : stmt := x <- (fun _ => 0);; Swhile tt (x <- incr_x).
 
 (* Proposition 5.2 *)
 Lemma prg_spec: forall (n:nat), semax ttS s (Eventually_x_is_n n).
-Proof. 
+Proof.
 move => n.
 have hs0: semax ttS (x <- (fun _ => 0))
 (Updt ttS x (fun _ => 0) *** [| x_is_zero |]).
 * have := semax_conseq_R _ (semax_assign _ _ _). apply.
   move => tr. simpl. move => h0. exists tr. split => //.
-  foo h0. destruct H as [_ h0]. foo h0. foo H1.
-  apply follows_delay. apply follows_nil => //. 
-  exists (update x 0 x0). split => //. rewrite /update.
-  have h: x =? x = true by apply Nat.eqb_refl.
-  by rewrite /x_is_zero h. by apply bisim_reflexive.
+  inv h0. destruct H as [_ h0]. inv h0. inv H1.
+  apply follows_delay. apply follows_nil => //.
+  exists (update x 0 x0). split => //.
+  + by rewrite /update /x_is_zero Nat.eqb_refl.
+  by apply: bisim_reflexive.
 have hs1 : semax x_is_zero (Swhile tt (x <- incr_x)) (Eventually_x_is_n n).
 have h0 := semax_assign ttS x incr_x.
-have h1 : (ttS andS eval_true tt) ->> ttS; first done.
-have h2 : (Updt ttS x incr_x) =>> (Updt ttS x incr_x) *** [| ttS |]. 
-* clear h0 h1. move => tr0 h0. exists tr0. split => //. clear h0. 
-  move: tr0. cofix hcoind. case. move => st0. apply follows_nil => //. 
-  have := mk_singleton_nil. apply. done. move => st0 tr0. 
-  have := follows_delay _ (hcoind tr0). apply. 
+have h1 : (ttS andS eval_true tt) ->> ttS by [].
+have h2 : (Updt ttS x incr_x) =>> (Updt ttS x incr_x) *** [| ttS |].
+* clear h0 h1. move => tr0 h0. exists tr0. split => //. clear h0.
+  move: tr0. cofix hcoind. case=> st0.
+  + apply follows_nil => //. by apply: (mk_singleton_nil).
+  move =>tr0.
+  by apply: (follows_delay _ (hcoind tr0)).
 have h3 := semax_conseq h1 h2 h0 => {h0 h1 h2}.
 have h0 : x_is_zero ->> ttS by [].
 have h1 := semax_while h0 h3 => {h0 h3}.
 have h0 : ((<< x_is_zero >>) ***
  Iter (Updt ttS x incr_x *** (<< ttS >>)) *** ([|eval_false tt|])) =>>
  (Eventually_x_is_n n).
-* clear h1. move => tr0 h0. move: h0 => [tr1 [h0 h1]]. move: h0 => [st0 [h0 h2]]. 
-  foo h2. foo H1. foo h1. foo H2. simpl.
+* clear h1. move => tr0 [tr1 [[st0 [h0 h2]] h1]].
+  inv h2. inv H1. inv h1. inv H2. simpl.
   have h1: forall n tr,
    append (iter (append (updt ttS x incr_x) (dup ttS)))
        (singleton (eval_false tt)) tr ->
    eventually_x_is_n (hd tr x + n) tr.
-  * clear H1 h0 n tr'. move => n. induction n. 
-    - case. move => st0 _. apply x_is_n_nil. simpl. by lia. 
-      move => st0 tr0 _. apply x_is_n_cons. simpl. by lia.
-    - move => tr0 h0. move: h0 => [tr1 [h0 h1]]. foo h0.
-      foo h1. move: H1 => [st0 [h0 _]]. rewrite /eval_false in h0.
-      rewrite tt_true in h0. foo h0. move: H => [tr2 [h0 h2]]. 
-      move: h0 => [st0 [_ h0]]. foo h0. foo H2. foo h2. 
-      foo H0. foo H3. move: H1 => [st1 [_ h2]]. foo h2. simpl in H0. 
-      foo H2. foo h1. foo H4. foo H3. foo H2. simpl. apply x_is_n_delay.
+  * clear H1 h0 n tr'. move => n. induction n.
+    - case=> st0.
+      + move =>_. apply x_is_n_nil. simpl. by lia.
+      move => tr0 _. apply x_is_n_cons. simpl. by lia.
+    - move => tr0 [tr1 [h0 h1]]. inv h0.
+      + inv h1. move: H1 => [st0 [h0 _]]. by rewrite /eval_false tt_true in h0.
+      move: H => [tr2 [[st0 [_ h0]] h2]].
+      inv h0. inv H2. inv h2. inv H0. inv H3.
+      move: H1 => [st1 [_ h2]]. inv h2. simpl in H0.
+      inv H2. inv h1. inv H4. inv H3. inv H2. simpl. apply x_is_n_delay.
       have h0 := follows_singleton H5.
       have h1: append (iter (append (updt ttS x incr_x) (dup ttS)))
        (singleton (eval_false tt)) tr'1.
-      exists tr'1; split; first done.
-      have := follows_setoid_R (@singleton_setoid _) H5 (bisim_symmetric h0).
-      by apply. have h2 := IHn _ h1 => {h1 H5}.
-      have h1: st0 x + S n = hd tr'1 x + n. 
-      rewrite H0. rewrite (update_x_incr_x st0). lia. 
-      rewrite h1 => {h1}. apply x_is_n_delay. 
-      have := eventually_x_is_n_setoid h2 h0. by apply. 
-  apply x_is_n_delay. have h2 := h1 _ _ H1 => {h1 H1}. 
-  foo h0. have h0: n = hd tr' x + n by rewrite H0; lia. rewrite h0 => {h0}.
-  by apply h2. 
-have := semax_conseq_R h0 h1. by apply. 
-have := semax_seq hs0 hs1 => {hs0 hs1}. move => hs. 
-have := semax_conseq_R _ hs => {hs}. apply. move => tr0. simpl.
-move => [tr1 [h0 h1]]. destruct h0 as [st0 [h0 h2]]. foo h2. foo H1.
-foo h1. foo H2. by apply x_is_n_delay.
+      + exists tr'1; split=>//.
+        by apply: (follows_setoid_R (@singleton_setoid _) H5 (bisim_symmetric h0)).
+      have h2 := IHn _ h1 => {h1 H5}.
+      have h1: st0 x + S n = hd tr'1 x + n
+        by rewrite H0 (update_x_incr_x st0); lia.
+      rewrite h1 => {h1}. apply x_is_n_delay.
+      by apply: (eventually_x_is_n_setoid h2 h0).
+  apply x_is_n_delay. have h2 := h1 _ _ H1 => {h1 H1}.
+  inv h0. have h0: n = hd tr' x + n by rewrite H0; lia. rewrite h0 => {h0}.
+  by apply h2.
+by apply: (semax_conseq_R h0 h1).
+move: (semax_seq hs0 hs1) => {hs0 hs1}hs.
+apply: (semax_conseq_R _ hs) => {hs} tr0 /= [tr1 [[st0 [h0 h2]] h1]].
+inv h2. inv H1. inv h1. inv H2. by apply x_is_n_delay.
 Qed.
