theories/Semax.v
@@ -11,7 +11,7 @@ Inductive semax : assertS -> stmt -> assertT -> Prop :=
 | semax_assign: forall u x a, semax u (Sassign x a) (Updt u x a)
 
 | semax_seq: forall s1 s2 u v p1 p2,
-  semax u s1 (p1 *** [|v|]) -> 
+  semax u s1 (p1 *** [|v|]) ->
   semax v s2 p2 ->
   semax u (Sseq s1 s2)  (p1 *** p2)
 
@@ -26,8 +26,8 @@ Inductive semax : assertS -> stmt -> assertT -> Prop :=
   semax u0 (Swhile a s) (<<u0>> *** (Iter (p *** <<u>>)) *** [|eval_false a|])
 
 | semax_conseq: forall s u1 u2 p1 p2,
-  u1 ->> u2 -> 
-  p2 =>> p1 -> 
+  u1 ->> u2 ->
+  p2 =>> p1 ->
   semax u2 s p2 ->
   semax u1 s p1
 
@@ -36,83 +36,88 @@ Inductive semax : assertS -> stmt -> assertT -> Prop :=
   semax (exS u) s (exT p).
 
 Lemma semax_conseq_R: forall u s p q,
-p =>> q -> semax u s p -> semax u s q. 
-Proof. 
-move => u s p q h0 h1. 
-have := semax_conseq (@assertS_imp_refl u) h0 h1. apply. 
-Qed.   
+p =>> q -> semax u s p -> semax u s q.
+Proof.
+move => u s p q h0 h1.
+by apply: (semax_conseq (@assertS_imp_refl u) h0 h1).
+Qed.
 
 Lemma semax_conseq_L: forall u v s p,
-v ->> u -> semax u s p -> semax v s p. 
-Proof. 
-move => u v s p h0 h1. 
-have := semax_conseq h0 _ h1.
-apply. done.   
-Qed.   
+v ->> u -> semax u s p -> semax v s p.
+Proof.
+move => u v s p h0 h1.
+by apply: (semax_conseq h0 _ h1).
+Qed.
 
 (* Lemma 3.5 *)
-Lemma push_pre: forall u s p, semax u s p -> semax u s ([|u|] *** p). 
-Proof. 
+Lemma push_pre: forall u s p, semax u s p -> semax u s ([|u|] *** p).
+Proof.
 have: forall u s p, semax u s p -> forall v, semax (u andS v) s ([|v|] *** p).
-induction 1. 
-- move => v. have := semax_conseq_R _ (semax_skip _). apply. 
-  move => tr0. simpl. move => [st0 [h0 h1]]. foo h1. exists (Tnil st0).
-  destruct h0 as [h0 h1]. split. exists st0. split => //. apply bisim_reflexive. 
-  apply follows_nil => //. exists st0. split => //. apply bisim_reflexive. 
-- move => v. have := semax_conseq_R _ (semax_assign _ _ _). apply. 
-  move => tr0. simpl. move => [st0 [h0 h1]]. foo h1. foo H1. 
-  destruct h0 as [h0 h1]. exists (Tnil st0). split. exists st0. split => //. 
-  apply bisim_reflexive. apply follows_nil => //. exists st0. split => //. 
-  apply bisim_reflexive. 
+induction 1.
+- move=>v; apply: (semax_conseq_R _ (semax_skip _)).
+  move=>tr0 /= [st0 [h0 h1]]. inv h1. exists (Tnil st0).
+  move: h0=>[h0 h1]. split.
+  - exists st0. split=>//. apply: bisim_reflexive.
+  apply follows_nil => //. exists st0. split => //. apply bisim_reflexive.
+- move => v. apply: (semax_conseq_R _ (semax_assign _ _ _)).
+  move => tr0 /= [st0 [h0 h1]]. inv h1. inv H1.
+  move: h0=>[h0 h1]. exists (Tnil st0). split.
+  - exists st0. split => //. apply bisim_reflexive.
+  apply follows_nil => //. exists st0. split => //.
+  apply bisim_reflexive.
 - move => v0. have hs1 := IHsemax1 v0 => {IHsemax1}.
   have hs2 := IHsemax2 v => {IHsemax2}.
-  have := semax_conseq_R (@Append_assoc_R _ _ _) hs1.
-  clear hs1. move => hs1. have := semax_conseq_R _ (semax_seq hs1 
-  (semax_conseq_L _ hs2)). apply.
-  have := assertT_imp_trans _ (@Append_assoc_L _ _ _). apply.
-  apply Append_monotone_R. apply Singleton_Append.      
-  move => st0 h0. split => //. 
+  move: (semax_conseq_R (@Append_assoc_R _ _ _) hs1) => {}hs1.
+  apply: (semax_conseq_R _ (semax_seq hs1 (semax_conseq_L _ hs2))).
+  - apply: (assertT_imp_trans _ (@Append_assoc_L _ _ _)).
+    apply Append_monotone_R. apply Singleton_Append.
+  by move => st0 h0.
 - move => v. have hs1 := IHsemax1 v => {IHsemax1}.
-  have h0: ((u andS v) andS eval_true a) ->> ((u andS eval_true a) andS v).
-  * move => st0 [[h0 h1] h2] => //.
-  have := semax_conseq_L h0 hs1 => {hs1}. move => hs1.   
-  have hs2 := IHsemax2 v => {IHsemax2}. clear h0. 
-  have h0: ((u andS v) andS eval_false a) ->> ((u andS eval_false a) andS v).
-  * move => st0 [[h0 h1] h2] => //.
-  have := semax_conseq_L h0 hs2 => {hs2}. move => hs2.
-  have := semax_ifthenelse hs1 hs2 => {hs1 hs2}. clear h0. move => h. 
-  have := semax_conseq_R _ h. apply. 
-  have := assertT_imp_trans (@Append_assoc_R _ _ _). apply.
-  have := assertT_imp_trans _ (@Append_assoc_L _ _ _). apply. 
-  apply Append_monotone_L. move => tr0. simpl. move => [tr1 [h0 h1]].
-  destruct h0 as [st0 [h0 h2]]. foo h2. foo H3. destruct h0 as [h0 h2]. 
-  foo h1. foo H4. destruct H3 as [st0 [h1 h3]]. foo h3. simpl in h0. simpl in h2. 
-  simpl. exists (Tnil st0). split. exists st0; split => //. apply bisim_reflexive. 
-  apply follows_nil => //. exists st0. split => //. apply bisim_reflexive. 
-- move => v. have := IHsemax ttS => {IHsemax}. 
-  move => hs. have hpre: (u andS eval_true a) ->> 
-  (u andS eval_true a) andS ttS. move => st0 [h0 h1]. split => //. 
-  have := semax_conseq_L hpre hs => {hs hpre}. move => hs. 
-  have := semax_conseq_R (@ttS_Chop _) hs => {hs}. move => hs. 
-  have := semax_conseq_R _ (semax_while _ hs). apply.
-  have := assertT_imp_trans _ (@Append_assoc_L _ _ _). apply.
-  apply Append_monotone_L. move => tr0 [st0 [h0 h1]]. destruct h0 as [h0 h2]. 
-  foo h1. foo H3. simpl. exists (Tnil st0). split. exists st0. split => //. 
-  apply bisim_reflexive. apply follows_nil => //. exists st0. split => //. 
-  apply bisim_reflexive. move => st0 [h0 h1]. have := H _ h0. done. 
-- move => v. have hs := IHsemax v => {IHsemax}. 
-  have := semax_conseq _ _ hs. apply. move => st0 [h0 h1].
-  split => //. have := H _ h0. done. apply Append_monotone_R. done. 
-- move => v. have hpre: (exS u andS v) ->> exS (fun x => u x andS v). 
-  * move => st0 [h0 h1]. destruct h0 as [x h0]. exists x. split => //. 
+  have h0: ((u andS v) andS eval_true a) ->> ((u andS eval_true a) andS v)
+    by move => st0 [[h0 h1] h2].
+  move: (semax_conseq_L h0 hs1) => {}hs1.
+  have hs2 := IHsemax2 v => {IHsemax2}. clear h0.
+  have h0: ((u andS v) andS eval_false a) ->> ((u andS eval_false a) andS v)
+   by move => st0 [[h0 h1] h2].
+  move: (semax_conseq_L h0 hs2) => {}hs2.
+  move: (semax_ifthenelse hs1 hs2) => {h0 hs1 hs2}h.
+  apply: (semax_conseq_R _ h).
+  apply: (assertT_imp_trans (@Append_assoc_R _ _ _)).
+  apply: (assertT_imp_trans _ (@Append_assoc_L _ _ _)).
+  apply: Append_monotone_L => tr0 /= [tr1 [h0 h1]].
+  move: h0 => [st0 [h0 h2]]. inv h2. inv H3. move: h0 => [h0 h2].
+  inv h1. inv H4. destruct H3 as [st0 [h1 h3]]. inv h3. simpl in h0. simpl in h2.
+  simpl. exists (Tnil st0). split. exists st0; split => //. apply bisim_reflexive.
+  apply follows_nil => //. exists st0. split => //. apply bisim_reflexive.
+- move => v.
+  move: (IHsemax ttS) => {IHsemax}hs.
+  have hpre: (u andS eval_true a) ->> (u andS eval_true a) andS ttS
+    by move => st0 [h0 h1]; split.
+  move: (semax_conseq_L hpre hs) => {hpre}hs.
+  move: (semax_conseq_R (@ttS_Chop _) hs) => {}hs.
+  apply: (semax_conseq_R _ (semax_while _ hs)).
+  * apply: (assertT_imp_trans _ (@Append_assoc_L _ _ _)).
+    apply: Append_monotone_L => tr0 [st0 [[h0 h2] h1]].
+    inv h1. inv H3. simpl. exists (Tnil st0). split.
+    + exists st0. split => //. apply bisim_reflexive.
+    apply follows_nil => //. exists st0. split => //.
+    apply bisim_reflexive.
+  move => st0 [h0 h1]. by apply: H.
+- move => v. have hs := IHsemax v => {IHsemax}.
+  apply: (semax_conseq _ _ hs).
+  * move => st0 [h0 h1]. split => //. by apply: H.
+  by apply Append_monotone_R.
+- move => v. have hpre: (exS u andS v) ->> exS (fun x => u x andS v).
+  * move => st0 [h0 h1]. destruct h0 as [x h0]. by exists x.
   have hpost: (exT (fun x => [|v|] *** p x)) =>> ([|v|] *** exT p).
-  * move => tr0 [x h0]. move hp: (p x) => px. rewrite hp in h0. 
-    destruct px as [q hq]. simpl in h0. destruct h0 as [tr1 [h0 h1]]. 
-    destruct h0 as [st0 [h0 h2]]. foo h2. foo h1. simpl. 
-    exists (Tnil (hd tr0)). split. exists (hd tr0). split => //.  apply bisim_reflexive. 
-    apply follows_nil => //. exists x. rewrite hp. simpl. done. 
-  have := semax_conseq hpre hpost. apply. apply semax_ex. 
-  clear hpre hpost. move => x. have := H0 _ v. done. 
-move => h u s p hs. have := h _ _ _ hs => {hs}. move => hs.
-have := semax_conseq_L _ (hs _). apply. done.
+  * move => tr0 [x h0]. move hp: (p x) => px. rewrite hp in h0.
+    destruct px as [q hq]. simpl in h0. destruct h0 as [tr1 [h0 h1]].
+    destruct h0 as [st0 [h0 h2]]. inv h2. inv h1. simpl.
+    exists (Tnil (hd tr0)). split.
+    + exists (hd tr0). split => //.  apply bisim_reflexive.
+    apply follows_nil => //. exists x. by rewrite hp.
+  apply: (semax_conseq hpre hpost). apply semax_ex.
+  clear hpre hpost. move => x. by apply: H0.
+move => h u s p hs. move: (h _ _ _ hs) => {}hs.
+by apply: (semax_conseq_L _ (hs _)).
 Qed.
