theories/SmallFunct.v
@@ -5,9 +5,9 @@ Unset Strict Implicit.
 Import Prenex Implicits.
 
 (* one-step reduction function *)
-Fixpoint red (s: stmt) (st: state) {struct s}: option (stmt * state) := 
+Fixpoint red (s: stmt) (st: state) {struct s}: option (stmt * state) :=
 match s with
-| Sskip => None 
+| Sskip => None
 | (Sassign x a) => Some (Sskip, update x (a st) st)
 | (Sseq s1 s2) =>
   match red s1 st with
@@ -17,116 +17,109 @@ match s with
 | (Sifthenelse a s1 s2) =>
   if is_true (a st) then Some (s1, st) else Some (s2, st)
 | (Swhile a s) =>
-  if is_true (a st)  then Some (Sseq s (Swhile a s), st) 
+  if is_true (a st)  then Some (Sseq s (Swhile a s), st)
   else Some (Sskip, st)
-end. 
+end.
 
 (* small-step functional semantics *)
 CoFixpoint Redm (s: stmt) (st: state): trace :=
 match red s st with
 | None => Tnil st
-| Some (s', st') => Tcons st (Redm s' st') 
+| Some (s', st') => Tcons st (Redm s' st')
 end.
 
 Lemma red_then_stop: forall s st,
-red s st = None -> stop s. 
-Proof. 
-move => s; induction s. 
-- move => st h1. by apply stop_skip. 
-- move => st h1. by inversion h1.  
-- move => st h1. foo h1. case_eq (red s1 st).  
-  - move => [s1'  st'] h2. rewrite h2 in H0. by inversion H0.  
-  - move => h2. rewrite h2 in H0. by have := stop_seq (IHs1 _ h2) (IHs2 _ H0); apply. 
-- move => st h1. foo h1.  case_eq (is_true (e st)); move => h2.
-  - rewrite h2 in H0. by inversion H0. 
-  - rewrite h2 in H0. by inversion H0. 
-- move => st h1. foo h1. case_eq (is_true (e st)); move => h2.
-  - rewrite h2 in H0. by inversion H0. 
-  - rewrite h2 in H0. by inversion H0.  
+red s st = None -> stop s.
+Proof.
+move=>s; induction s=>st h1.
+- by apply: stop_skip.
+- by inversion h1.
+- inv h1. case h2 : (red s1 st) =>[[??]|]; rewrite h2 // in H0.
+  by apply: (stop_seq (IHs1 _ h2) (IHs2 _ H0)).
+- inv h1. move: H0. by case: (is_true (e st)).
+- inv h1. move: H0. by case: (is_true (e st)).
 Qed.
 
 Lemma red_then_step: forall s st s' st',
 red s st = Some (s', st') -> step s st s' st'.
-Proof. 
-move => s; induction s. 
-- move => st s st' h1. by inversion h1.  
-- move => st s st' h1. foo h1. by apply step_assign. 
-- move => st1 s3 st2 h1. case_eq (red s1 st1).  
-  - move => [s1' st1'] h2. foo h1. rewrite h2 in H0. foo H0.   
-    apply: step_seq1. by have := IHs1 _ _ _ h2; apply.   
-  - move => h2. foo h1. rewrite h2 in H0. 
-    by have := step_seq2 (red_then_stop h2) (IHs2 _ _ _ H0); apply.   
-- move => st1 s3 st2 h1. case_eq (is_true (e st1)) => h2.
-  - simpl in h1. rewrite h2 in h1. foo h1.
-    apply: step_ifthenelse_true. by apply h2. 
-  - simpl in h1. rewrite h2 in h1. foo h1.  
-    apply: step_ifthenelse_false. by apply h2. 
-- move => st s' st' h1. case_eq (is_true (e st)) => h2. 
-  - simpl in h1. rewrite h2 in h1. foo h1. apply: step_while_true. 
-    by apply h2.  
-  - simpl in h1. rewrite h2 in h1. foo h1. 
-    apply: step_while_false. by apply h2.  
-Qed.
-
-Lemma stop_then_red: forall s st, stop s -> red s st = None. 
 Proof.
-induction 1. 
-- by simpl.
-- simpl. rewrite IHstop1. by apply IHstop2. 
-Qed. 
-
-Lemma step_then_red: forall s st s' st', 
-step s st s' st' -> red s st = Some (s', st').
-Proof. 
-induction 1. 
-- by simpl.
-- simpl. rewrite IHstep. simpl. done. 
-- simpl. have h1 := stop_then_red st H. rewrite h1. rewrite IHstep. done. 
-- simpl. rewrite H. done. 
-- simpl. by rewrite H. 
-- simpl. by rewrite H.
-- simpl. by rewrite H. 
+move => s; induction s.
+- move => st s st' h1. by inversion h1.
+- move => st s st' h1. inv h1. by apply step_assign.
+- move => st1 s3 st2 h1. case h2 : (red s1 st1)=> [[s1' st1']|].
+  - inv h1. rewrite h2 in H0. inv H0.
+    by apply/step_seq1/IHs1.
+  - inv h1. rewrite h2 in H0.
+    by apply: (step_seq2 (red_then_stop h2) (IHs2 _ _ _ H0)).
+- move => st1 s3 st2 /= h1. case/boolP: (is_true (e st1))=>h2.
+  - rewrite h2 in h1. inv h1.
+    by apply: step_ifthenelse_true.
+  - rewrite (negbTE h2) in h1. inv h1.
+    by apply: step_ifthenelse_false.
+- move => st s' st' /= h1. case/boolP: (is_true (e st)) => h2.
+  - rewrite h2 in h1. inv h1.
+    by apply: step_while_true.
+  - rewrite (negbTE h2) in h1. inv h1.
+    by apply: step_while_false.
 Qed.
- 
+
+Lemma stop_then_red: forall s st, stop s -> red s st = None.
+Proof.
+induction 1=>//=.
+by rewrite IHstop1.
+Qed.
+
+Lemma step_then_red: forall s st s' st',
+step s st s' st' -> red s st = Some (s', st').
+Proof.
+induction 1=>//=.
+- by rewrite IHstep.
+- by rewrite (stop_then_red st H) IHstep.
+- by rewrite H.
+- by rewrite (negbTE H).
+- by rewrite (negbTE H).
+- by rewrite H.
+Qed.
+
 (* the small-step functional semantics correct wrt the small-step relational semantics. *)
 Lemma Redm_correct_redm: forall st s, redm s st (Redm s st).
 Proof.
-cofix COINDHYP. move => st s. rewrite [Redm s st]trace_destr.
-simpl. case_eq (red s st). 
-- move => [s' st'] h1. simpl. have h2 := red_then_step h1. 
-  have := redm_step h2; apply. by apply COINDHYP.
-- move => h1. apply redm_stop. by have := red_then_stop h1; apply.  
+cofix COINDHYP=>st s. rewrite [Redm s st]trace_destr /=.
+case h1 : (red s st) => [[s' st'] /=|].
+- have h2 := red_then_step h1.
+  by apply/(redm_step h2)/COINDHYP.
+- by apply/redm_stop/(red_then_stop h1).
 Qed.
 
 (* the small-step relational semantics correct wrt the small-step functional semantics *)
 Lemma redm_correct_Redm: forall s st tr, redm s st tr -> bisim tr (Redm s st).
-Proof. 
-move => s st tr h1. have h2 := Redm_correct_redm st s. 
-by have := redm_deterministic h1 h2; apply. 
-Qed.   
+Proof.
+move => s st tr h1.
+have h2 := Redm_correct_redm st s.
+by apply: (redm_deterministic h1 h2).
+Qed.
 
 Lemma redmseq_correct_execseq0: forall s,
 (forall st tr, redm s st tr -> exec s st tr) ->
 forall tr1 tr2, redm_str s tr1 tr2 ->
 execseq s tr1 tr2.
 Proof.
-move => s h. cofix COINDHYP. move => tr1 tr2 h1. foo h1.  
-- by have := execseq_nil (h _ _ H); apply.  
-- by have := execseq_cons _  (COINDHYP _ _ H); apply. 
+move => s h.
+cofix COINDHYP => tr1 tr2 h1. inv h1.
+- by apply/execseq_nil/h.
+- by apply/execseq_cons/COINDHYP.
 Qed.
 
 Lemma Redm_sequence: forall s1 s2 st,
 bisim (Redm (Sseq s1 s2) st) (sequence (Redm s2) (Redm s1 st)).
 Proof.
-cofix COINDHYP. move => s1 s2 st. 
-rewrite [Redm (Sseq s1 s2) st]trace_destr; simpl.  
-rewrite [Redm s1 st]trace_destr; simpl. case_eq (red s1 st). 
-- move => [s1' st'] h1. rewrite [sequence _ _]trace_destr; simpl. 
-  by have := bisim_cons _(COINDHYP _ _ _); apply. 
-- move => h1.  rewrite [sequence _ _]trace_destr; simpl. 
-  case_eq (red s2 st).
-  - move => *. by apply bisim_reflexive. 
-  - move => *.  by apply bisim_nil. 
+cofix COINDHYP=> s1 s2 st.
+rewrite [Redm (Sseq s1 s2) st]trace_destr /= [Redm s1 st]trace_destr /=.
+case h1 : (red s1 st) => [[s1' st']|]; rewrite [sequence _ _]trace_destr /=.
+- by apply/bisim_cons/COINDHYP.
+- case: (red s2 st)=>*.
+  - by apply: bisim_reflexive.
+  - by apply: bisim_nil.
 Qed.
 
 
@@ -135,129 +128,116 @@ Lemma sequence_deterministic0: forall k1 k2,
 forall tr1 tr2, bisim tr1 tr2 ->
 bisim (sequence k1 tr1) (sequence k2 tr2).
 Proof.
-move => k1 k2 h1. cofix COINDHYP. move => tr1 tr2 h2. foo h2. 
-- rewrite [sequence k1 _]trace_destr. 
-  rewrite [sequence k2 _]trace_destr; simpl. 
-  have h3 := h1 st. foo h3.
-  - by apply bisim_nil. 
-  - by have := bisim_cons _ H1; apply. 
-- rewrite [sequence k1 _]trace_destr; simpl. 
-  rewrite [sequence k2 _]trace_destr; simpl. 
-  by have := bisim_cons  _ (COINDHYP _ _ H); apply. 
-Qed. 
+move => k1 k2 h1.
+cofix COINDHYP=> tr1 tr2 h2. inv h2.
+- rewrite [sequence k1 _]trace_destr [sequence k2 _]trace_destr /=.
+  have h3 := h1 st.
+  inv h3; first by apply: bisim_nil.
+  by apply: bisim_cons.
+- rewrite [sequence k1 _]trace_destr /= [sequence k2 _]trace_destr /=.
+  by apply/bisim_cons/COINDHYP.
+Qed.
 
 Lemma Redm_loop_skip: forall a s st,
 is_true (a st) = true ->
 red s st = None ->
 bisim (Redm (Sseq s (Swhile a s)) st)
  (loop (Redm s) (fun st0 => is_true (a st0)) st).
-Proof. 
-move => a s st h1 h2. cofix COINDHYP. 
-rewrite [Redm _ _]trace_destr; simpl. 
-rewrite [loop _ _ _]trace_destr; simpl.
-rewrite h1; rewrite h2; simpl.
-by have := bisim_cons _ COINDHYP; apply. 
-Qed.  
+Proof.
+move => a s st h1 h2.
+cofix COINDHYP.
+rewrite [Redm _ _]trace_destr /= [loop _ _ _]trace_destr /= h1 h2 /=.
+by apply/bisim_cons/COINDHYP.
+Qed.
 
 
 Lemma Redm_loop: forall a s,
-forall st, bisim (Redm (Swhile a s) st) 
+forall st, bisim (Redm (Swhile a s) st)
  (Tcons st (loop (Redm s) (fun st0 => is_true (a st0)) st)).
 Proof.
-cofix COINDHYP. 
-have COINDHYP2: forall a s s1 st1, 
+cofix COINDHYP.
+have COINDHYP2: forall a s s1 st1,
 bisim (Redm (Sseq s1 (Swhile a s)) st1)
-(loopseq (Redm s) (fun st0 => is_true (a st0)) (Redm s1 st1)). 
+(loopseq (Redm s) (fun st0 => is_true (a st0)) (Redm s1 st1)).
 * cofix COINDHYP2. move => a s s1 st1. case_eq (red s1 st1).
-  - move => [s1' st1'] h1. rewrite [loopseq _ _ _]trace_destr; simpl. 
-    rewrite [Redm _ _]trace_destr; simpl. rewrite h1. simpl. 
-    by have := bisim_cons _ (COINDHYP2 _ _ _ _); apply.   
+  - move => [s1' st1'] h1.
+    rewrite [loopseq _ _ _]trace_destr /= [Redm _ _]trace_destr /= h1 /=.
+    by apply/bisim_cons/COINDHYP2.
   - move => h1. case_eq (is_true (a st1)) => h2.
-    - rewrite [Redm _ _]trace_destr; simpl. rewrite h1. rewrite h2. simpl. 
-      rewrite [loopseq _ _ _]trace_destr; simpl. rewrite h1. 
-      rewrite [loop _ _ _]trace_destr; simpl. rewrite h2. 
-      case_eq (red s st1). 
-      - move => [s' st1'] h3. rewrite [Redm _ _]trace_destr; simpl. 
-        rewrite h3. simpl. by have := bisim_cons _ (bisim_cons _ (COINDHYP2 _ _ _ _)); apply.  
-      - move => h3. rewrite [Redm _ _]trace_destr; simpl. rewrite h2; rewrite h3; simpl. 
-        by apply: (bisim_cons _ (bisim_cons _ (Redm_loop_skip h2 h3))).
-    - rewrite [Redm _ _]trace_destr; simpl. rewrite h1; rewrite h2; simpl.
-      rewrite [loopseq _ _ _]trace_destr; simpl. rewrite h1; simpl. 
-      rewrite [loop _ _ _]trace_destr; simpl. rewrite h2; simpl.
-      rewrite [Redm _ _]trace_destr; simpl. by apply bisim_reflexive. 
+    - rewrite [Redm _ _]trace_destr /= h1 h2 /= [loopseq _ _ _]trace_destr /= h1 /=
+              [loop _ _ _]trace_destr /= h2.
+      case_eq (red s st1).
+      - move => [s' st1'] h3. rewrite [Redm _ _]trace_destr /= h3 /=.
+        by apply/bisim_cons/bisim_cons/COINDHYP2.
+      - move => h3. rewrite [Redm _ _]trace_destr /= h2 h3 /=.
+        by apply/bisim_cons/bisim_cons/(Redm_loop_skip h2 h3).
+    - rewrite [Redm _ _]trace_destr /= h1 h2 /= [loopseq _ _ _]trace_destr /= h1 /=
+              [loop _ _ _]trace_destr /= h2 /= [Redm _ _]trace_destr /=.
+      by apply: bisim_reflexive.
 * move => a s st. case_eq (is_true (a st)) => h1.
-  - rewrite [Redm _ _]trace_destr; simpl. rewrite h1. simpl.
-    case_eq (red s st). 
-    - move => [s' st'] h2. 
-      rewrite [loop _ _ _]trace_destr; simpl. rewrite h1; rewrite h2; simpl.
-      rewrite [Redm _ _]trace_destr; simpl. rewrite h2; simpl. 
-      by apply: (bisim_cons _ (bisim_cons _ (COINDHYP2 _ _ _ _))).
-    - move => h2. by apply: (bisim_cons _ (Redm_loop_skip h1 h2)).
-  - rewrite [Redm _ _]trace_destr; simpl. rewrite h1; simpl. 
-    rewrite [Redm _ _]trace_destr; simpl. 
-    rewrite [loop _ _ _]trace_destr; simpl. rewrite h1; simpl. 
-    by apply bisim_reflexive. 
-Qed.   
+  - rewrite [Redm _ _]trace_destr /= h1 /=.
+    case_eq (red s st).
+    - move => [s' st'] h2.
+      rewrite [loop _ _ _]trace_destr /= h1 h2 /= [Redm _ _]trace_destr /= h2 /=.
+      by apply/bisim_cons/bisim_cons/COINDHYP2.
+    - move => h2. by apply/bisim_cons/(Redm_loop_skip h1 h2).
+  - rewrite [Redm _ _]trace_destr /= h1 /= [Redm _ _]trace_destr /=
+            [loop _ _ _]trace_destr /= h1 /=.
+    by apply: bisim_reflexive.
+Qed.
 
 Lemma loop_deterministic0: forall k1 k2 p,
 (forall st, bisim (k1 st) (k2 st)) ->
 forall st, bisim (loop k1 p st) (loop k2 p st).
-Proof. 
-move => k1 k2 p h1.  cofix COINDHYP. 
-have COINDHYP2:forall tr1 tr2,
-bisim tr1 tr2 -> bisim (loopseq k1 p tr1) (loopseq k2 p tr2).
-- cofix COINDHYP2. move => tr1 tr2 h2. foo h2. 
-  - rewrite [loopseq k1 _ _]trace_destr; simpl. 
-    rewrite [loopseq k2 _ _]trace_destr; simpl. 
-    by apply: (bisim_cons _ (COINDHYP _)). 
-  - rewrite [loopseq k1 _ _]trace_destr; simpl. 
-    rewrite [loopseq k2 _ _]trace_destr; simpl. 
-    by apply: (bisim_cons _ (COINDHYP2 _ _ H)). 
-* move => st. case_eq (p st) => h2.
-  - have h3 := h1 st. foo h3. 
-    - rewrite [loop k1 _ _]trace_destr; simpl.
-      rewrite [loop k2 _ _]trace_destr; simpl. 
-      rewrite h2; rewrite - H; rewrite -H0. 
-      by apply: (bisim_cons _ (COINDHYP _)). 
-    - rewrite [loop k1 _ _]trace_destr; simpl.
-      rewrite [loop k2 _ _]trace_destr; simpl. 
-      rewrite h2; rewrite - H; rewrite -H0. 
-      by apply: (bisim_cons _ (COINDHYP2 _ _ H1)).
-  - rewrite [loop k1 _ _]trace_destr; simpl.
-    rewrite [loop k2 _ _]trace_destr; simpl. rewrite h2. 
-    by apply bisim_nil. 
-Qed.  
+Proof.
+move => k1 k2 p h1. cofix COINDHYP.
+have COINDHYP2 : forall tr1 tr2,
+                 bisim tr1 tr2 -> bisim (loopseq k1 p tr1) (loopseq k2 p tr2).
+- cofix COINDHYP2=> tr1 tr2 h2. inv h2.
+  - rewrite [loopseq k1 _ _]trace_destr /= [loopseq k2 _ _]trace_destr /=.
+    by apply/bisim_cons/COINDHYP.
+  - rewrite [loopseq k1 _ _]trace_destr /= [loopseq k2 _ _]trace_destr /=.
+    by apply/bisim_cons/COINDHYP2.
+* move => st. case h2: (p st).
+  - have h3 := h1 st. inv h3.
+    - rewrite [loop k1 _ _]trace_destr /= [loop k2 _ _]trace_destr /= h2 -H -H0.
+      by apply/bisim_cons/COINDHYP.
+    - rewrite [loop k1 _ _]trace_destr /= [loop k2 _ _]trace_destr /= h2 -H -H0.
+      by apply/bisim_cons/COINDHYP2.
+  - rewrite [loop k1 _ _]trace_destr /= [loop k2 _ _]trace_destr /= h2.
+    by apply: bisim_nil.
+Qed.
 
 (* equivalence of the small-step functional semantics to the big-step functional semantics *)
 Lemma Exec_Redm: forall s st, bisim (Exec s st) (Redm s st).
-Proof. 
-move => s; induction s. 
-- move => st. rewrite [Redm _ _]trace_destr. simpl. by apply bisim_nil. 
-- move => st. rewrite [Redm _ _]trace_destr. simpl. 
-  rewrite [Redm _ _]trace_destr; simpl. by apply: (bisim_cons _ (bisim_nil _)).
-- move => st. simpl. have h1 := IHs1 st. 
-  have h2 := sequence_deterministic0 IHs2 h1. 
+Proof.
+move => s; induction s=>st.
+- rewrite [Redm _ _]trace_destr /=. by apply: bisim_nil.
+- rewrite [Redm _ _]trace_destr /= [Redm _ _]trace_destr /=.
+  by apply/bisim_cons/bisim_nil.
+- move => /=. have h1 := IHs1 st.
+  have h2 := sequence_deterministic0 IHs2 h1.
   have h3 := Redm_sequence s1 s2 st.
-  by apply: (bisim_transitive h2 (bisim_symmetric h3)).  
-- move => st. case_eq (is_true (e st)) => h1.
-  - rewrite [Redm _ _]trace_destr; simpl. rewrite h1; simpl.
-    by apply: (bisim_cons _ (IHs1 _)).  
-  - rewrite [Redm _ _]trace_destr; simpl. rewrite h1; simpl.
-    by apply: (bisim_cons _ (IHs2 _)).
-- move => st. simpl. have h1 := Redm_loop e s st.
+  by apply: (bisim_transitive h2 (bisim_symmetric h3)).
+- case h1: (is_true (e st)).
+  - rewrite [Redm _ _]trace_destr /= h1 /=.
+    by apply/bisim_cons/IHs1.
+  - rewrite [Redm _ _]trace_destr /= h1 /=.
+    by apply/bisim_cons/IHs2.
+- move => /=. have h1 := Redm_loop e s st.
   have h2 := loop_deterministic0 (fun st0 => is_true (e st0)) IHs st.
-  by apply: (bisim_symmetric (bisim_transitive h1 (bisim_cons _ (bisim_symmetric h2)))). 
-Qed. 
+  by apply/bisim_symmetric: (bisim_transitive h1 (bisim_cons _ (bisim_symmetric h2))).
+Qed.
 
-(* the small-step relational semantics correct wrt the big-step relational semantics *) 
+(* the small-step relational semantics correct wrt the big-step relational semantics *)
 (* by going through the functional semantics *)
 Lemma redm_correct_exec: forall s st tr, redm s st tr -> exec s st tr.
 Proof.
-move => s st tr h1. 
-have h2 := Redm_correct_redm st s. 
-have h3 := redm_deterministic h1 h2. 
-have h4 := Exec_Redm s st. 
+move => s st tr h1.
+have h2 := Redm_correct_redm st s.
+have h3 := redm_deterministic h1 h2.
+have h4 := Exec_Redm s st.
 have h5 := Exec_correct_exec s st.
-by have := exec_insensitive h5 (bisim_transitive h4 (bisim_symmetric h3)); apply. 
-Qed.  
+by apply: (exec_insensitive h5 (bisim_transitive h4 (bisim_symmetric h3))).
+Qed.
 
