theories/SsrExport.v
@@ -1,4 +1,4 @@
-From Coq Require Export ssreflect.
+From Coq Require Export ssreflect ssrfun ssrbool.
 Global Set SsrOldRewriteGoalsOrder.
 Global Set Asymmetric Patterns.
 Global Set Bullet Behavior "None".
