theories/Trace.v
@@ -4,25 +4,26 @@ Set Implicit Arguments.
 Unset Strict Implicit.
 Import Prenex Implicits.
 
-Ltac foo h := inversion h; subst => {h}.
+Ltac inv h := inversion h; subst => {h}.
 
 Definition id := nat.
 Definition val := nat.
-Definition state := id -> val. 
+Definition state := id -> val.
 
 CoInductive trace : Set :=
 | Tnil (_: state)
 | Tcons (_: state) (_: trace).
 
+(* AKA Chlipala's frob *)
 Definition trace_decompose (tr: trace): trace :=
 match tr with
 | Tnil st => Tnil st
 | Tcons a tr' => Tcons a tr'
-end. 
+end.
 
 Lemma trace_destr:
 forall tr, tr = trace_decompose tr.
-Proof. case => //=. Qed.  
+Proof. by case=>/=. Qed.
 
 (* bisimilarity of two traces *)
 CoInductive bisim: trace -> trace -> Prop :=
@@ -32,68 +33,75 @@ CoInductive bisim: trace -> trace -> Prop :=
   bisim tr tr' ->
   bisim (Tcons e tr) (Tcons e tr').
 
-(* Bisimilarity is reflexive *) 
-Lemma bisim_reflexive: forall tr, bisim tr tr. 
-Proof. 
-cofix COINDHYP. case.
-- move => st. by apply bisim_nil. 
-- move => st tr. by have := bisim_cons _ (COINDHYP _); apply.  
-Qed. 
+(* Bisimilarity is reflexive *)
+Lemma bisim_reflexive: forall tr, bisim tr tr.
+Proof.
+cofix CIH. case=>st.
+- by apply: bisim_nil.
+- by move=>?; apply/bisim_cons/CIH.
+Qed.
 
 (* Bisimilarity is symmetric *)
-Lemma bisim_symmetric: forall tr1 tr2, bisim tr1 tr2 -> bisim tr2 tr1. 
+Lemma bisim_symmetric: forall tr1 tr2, bisim tr1 tr2 -> bisim tr2 tr1.
 Proof.
-cofix COINDHYP. case. 
-- move => s tr2 h1. foo h1.  by apply: bisim_nil.  
-- move => s tr0 tr1 h1. foo h1. 
-  by have := bisim_cons _ (COINDHYP _ _ H2); apply.
-Qed.   
+cofix CIH. case=>s.
+- move=>? h1; inv h1.
+  by apply: bisim_nil.
+- move=>?? h1; inv h1.
+  by apply/bisim_cons/CIH.
+Qed.
 
-(* Bisimilarity is trnasitive *)
+(* Bisimilarity is transitive *)
 Lemma bisim_transitive: forall tr1 tr2 tr3,
-bisim tr1 tr2 -> bisim tr2 tr3 -> bisim tr1 tr3. 
+bisim tr1 tr2 -> bisim tr2 tr3 -> bisim tr1 tr3.
 Proof.
-cofix COINDHYP. case.  
-- move => st tr0 tr1 h1 h2. foo h1. foo h2. by apply: bisim_nil.
-- move => st tr0 tr1 tr2 h1 h2. foo h1. foo h2. 
-  by have := bisim_cons _ (COINDHYP _ _ _ H2 H3); apply.  
-Qed.    
+cofix CIH. case=>st tr0 tr1.
+- move=>h1 h2; inv h1; inv h2.
+  by apply: bisim_nil.
+- move=>? h1 h2; inv h1; inv h2.
+  by apply/bisim_cons/(CIH _ _ _ H2).
+Qed.
 
 
 CoFixpoint trace_append (tr tr': trace): trace :=
 match tr with
 | Tnil st => tr'
 | Tcons e tr0 => Tcons e (trace_append tr0 tr')
-end. 
+end.
 
 Infix "+++" := trace_append (at level 60, right associativity).
 
 Lemma trace_append_nil: forall st tr,
 (Tnil st) +++ tr = tr.
-Proof. 
-move => st tr. rewrite [Tnil st +++ tr]trace_destr. by case tr; simpl. 
-Qed. 
-   
+Proof.
+move=>st tr.
+rewrite [Tnil st +++ tr]trace_destr.
+by case: tr=>/=.
+Qed.
+
 Lemma trace_append_cons: forall e tr tr',
 (Tcons e tr) +++ tr' = Tcons e (tr +++ tr').
 Proof.
-move => st tr tr'. rewrite [Tcons st tr +++ tr']trace_destr. by case tr; simpl.
+move=>st tr tr'.
+rewrite [Tcons st tr +++ tr']trace_destr.
+by case: tr=>/=.
 Qed.
 
-Lemma trace_eq_append: forall tr1 tr2 tr3 tr4, 
+Lemma trace_eq_append: forall tr1 tr2 tr3 tr4,
 bisim tr1 tr2 -> bisim tr3 tr4 -> bisim (tr1 +++ tr3) (tr2 +++ tr4).
-Proof. 
-cofix COINDHYP. case. 
-- move => st1 tr1 tr2 tr3 h1 h2. foo h1.
-  do 2 rewrite trace_append_nil. by apply: h2. 
-- move => st tr1 tr2 tr3 tr4 h1 h2. foo h1. 
-  do 2 rewrite trace_append_cons.
-  have := bisim_cons _ (COINDHYP _ _ _ _ H2 h2); apply.
-Qed. 
+Proof.
+cofix CIH. case=>st1 tr1 tr2 tr3.
+- move=>h1 h2; inv h1.
+  by rewrite 2!trace_append_nil.
+- move=>tr4 h1 h2; inv h1.
+  rewrite 2!trace_append_cons.
+  by apply/bisim_cons/CIH.
+Qed.
 
-Definition hd tr := match tr with Tnil st => st | Tcons st tr0 => st end. 
+Definition hd tr := match tr with Tnil st => st | Tcons st tr0 => st end.
 
-Lemma bisim_hd: forall tr0 tr1, bisim tr0 tr1 -> hd tr0 = hd tr1. 
-Proof. 
-move => tr0 tr1 h0. by foo h0; simpl. 
+Lemma bisim_hd: forall tr0 tr1, bisim tr0 tr1 -> hd tr0 = hd tr1.
+Proof.
+move=>?? h0.
+by inv h0=>/=.
 Qed.
