theories/Weakbism.v
@@ -22,39 +22,36 @@ Definition decr_y: expr := fun st => st y - 1.
 
 Inductive red_hd_x : trace -> trace -> Prop :=
 | red_hd_x_stop: forall st tr tr',
-  st x <> hd tr x -> 
-  bisim tr tr' -> 
+  st x <> hd tr x ->
+  bisim tr tr' ->
   red_hd_x (Tcons st tr) tr'
 | red_hd_x_tau: forall st tr tr',
-  st x = hd tr x -> 
-  red_hd_x tr tr' -> 
+  st x = hd tr x ->
+  red_hd_x tr tr' ->
   red_hd_x (Tcons st tr) tr'.
 
 Lemma red_hd_x_deterministic: forall tr0 tr1, red_hd_x tr0 tr1 ->
-forall tr2, red_hd_x tr0 tr2 -> bisim tr1 tr2. 
-Proof. 
+forall tr2, red_hd_x tr0 tr2 -> bisim tr1 tr2.
+Proof.
 induction 1.
-- move => tr0 h0. foo h0. 
-  - have := bisim_transitive (bisim_symmetric H0) H5. by apply. 
-  - done. 
-- move => tr0 h0. foo h0. 
-  - done. 
-  - have := IHred_hd_x _ H5. by apply. 
+- move => tr0 h0. inv h0=>//.
+  by apply: (bisim_transitive (bisim_symmetric H0) H5).
+- move => tr0 h0. inv h0=>//.
+  by apply: (IHred_hd_x _ H5).
 Qed.
 
 Lemma red_hd_x_setoid: forall tr0 tr1, red_hd_x tr0 tr1 ->
-forall tr2, bisim tr0 tr2 -> forall tr3, bisim tr1 tr3 -> red_hd_x tr2 tr3. 
-Proof. 
-induction 1. 
-- move => tr0 h0 tr1 h2. foo h0. have h0 := bisim_hd H4. 
-  rewrite h0 in H => {h0}.
-  have := red_hd_x_stop H (bisim_transitive (bisim_transitive (bisim_symmetric H4) H0) h2).
-  by apply.
-- move => tr0 h0 tr1 h1. foo h0. have h2 := bisim_hd H4. 
-  rewrite h2 in H => {h2}. 
-  have := red_hd_x_tau H. apply. have := IHred_hd_x _ H4 _ h1. by apply. 
+forall tr2, bisim tr0 tr2 -> forall tr3, bisim tr1 tr3 -> red_hd_x tr2 tr3.
+Proof.
+induction 1.
+- move => tr0 h0 tr1 h2. inv h0.
+  rewrite (bisim_hd H4) in H.
+  by apply: (red_hd_x_stop H (bisim_transitive (bisim_transitive (bisim_symmetric H4) H0) h2)).
+- move => tr0 h0 tr1 h1. inv h0.
+  rewrite (bisim_hd H4) in H.
+  apply: (red_hd_x_tau H). by apply: (IHred_hd_x _ H4 _ h1).
 Qed.
- 
+
 CoInductive up : nat -> trace -> Prop :=
 | up_intro: forall st n tr0 tr1,
   st x = n ->
@@ -64,44 +61,43 @@ CoInductive up : nat -> trace -> Prop :=
 Lemma up_setoid: forall n tr0, up n tr0 ->
 forall tr1, bisim tr0 tr1 -> up n tr1.
 Proof.
-move => n tr0 h0 tr1 h1. foo h0. 
-foo h1. 
+move => n tr0 h0 tr1 h1. inv h0.
+inv h1.
 have h1 := red_hd_x_setoid H0 (bisim_cons st H4) (bisim_reflexive tr3).
-have := up_intro (refl_equal (st x)) h1 H1.
-by apply. 
+by apply: (up_intro (refl_equal (st x)) h1 H1).
 Qed.
 
-Definition Up (n:nat): assertT. 
-exists (fun tr => up n tr). 
+Definition Up (n:nat): assertT.
+exists (fun tr => up n tr).
 move => tr0 h0 tr1 h1.
-have := up_setoid h0 h1. by apply. 
-Defined.  
+have := up_setoid h0 h1. by apply.
+Defined.
 
 Inductive skips: trace -> Prop :=
 | skips_nil: forall st, skips (Tnil st)
 | skips_delay: forall st tr,
-  skips tr -> hd tr x = st x -> skips (Tcons st tr). 
+  skips tr -> hd tr x = st x -> skips (Tcons st tr).
 
 Lemma skips_setoid: forall tr0, skips tr0 -> forall tr1, bisim tr0 tr1 ->
-skips tr1. 
+skips tr1.
 Proof.
-induction 1. 
-- move => st0 h0. foo h0. by apply skips_nil.
-- move => tr0 h0. foo h0. apply skips_delay. 
+induction 1.
+- move => st0 h0. inv h0. by apply skips_nil.
+- move => tr0 h0. inv h0. apply skips_delay.
   have := IHskips _ H4. by apply. have h0 := bisim_hd H4.
-  rewrite -h0. done. 
-Qed. 
+  rewrite -h0. done.
+Qed.
 
 Definition Skips: assertT.
-exists (fun tr => skips tr). 
-move => tr0 h0 tr1 h1. simpl. 
-have := skips_setoid h0 h1. by apply. 
+exists (fun tr => skips tr).
+move => tr0 h0 tr1 h1. simpl.
+have := skips_setoid h0 h1. by apply.
 Defined.
 
-Lemma Sn_1 : forall n, S n - 1 = n. 
-Proof. by move => n; lia. Qed.  
+Lemma Sn_1 : forall n, S n - 1 = n.
+Proof. by move => n; lia. Qed.
 
-Lemma Sn: forall n, n + 1 = S n. 
+Lemma Sn: forall n, n + 1 = S n.
 Proof. by move => n; lia. Qed.
 
 Definition x_is_zero : assertS := fun st => st x = 0.
@@ -121,96 +117,96 @@ Definition s : stmt :=
 
 (* Proposition 5.3 *)
 Lemma spec: semax x_is_zero s (Up 0).
-Proof. 
-rewrite /s. 
+Proof.
+rewrite /s.
 pose a_t := eval_true cond.
-pose a_f := eval_false cond. 
-pose u_xy := fun st: state => st x = st y.      
+pose a_f := eval_false cond.
+pose u_xy := fun st: state => st x = st y.
 have h0 := semax_assign (ttS andS a_t) y decr_y.
 have h1 := semax_conseq_R (@Append_ttS _) h0 => {h0}.
 have h0: ttS ->> ttS; first done.
-have h2 := semax_while h0 h1 => {h0 h1}. 
+have h2 := semax_while h0 h1 => {h0 h1}.
 have h0 : ((<< ttS >>) *** Iter (Updt (ttS andS a_t) y decr_y *** (<< ttS >>)) ***
  [|eval_false cond|]) =>> Skips.
-* clear h2. move => tr0 h0. simpl. simpl in h0. move h1: (hd tr0 y) => n. 
-  move: tr0 h1 h0. induction n. 
-  - move => tr0 h0 [tr1 [h1 h2]]. move: h1 => [st0 [_ h1]]. foo h1. foo H1. 
-    foo h2. simpl in h0. foo H2. move: H1 => [tr0 [h1 h2]]. foo h1. 
-    - foo h2. move: H1 => [st0 [_ h1]]. foo h1. simpl. apply skips_delay. 
-      by apply skips_nil. by simpl. 
+* clear h2. move => tr0 h0. simpl. simpl in h0. move h1: (hd tr0 y) => n.
+  move: tr0 h1 h0. induction n.
+  - move => tr0 h0 [tr1 [h1 h2]]. move: h1 => [st0 [_ h1]]. inv h1. inv H1.
+    inv h2. simpl in h0. inv H2. move: H1 => [tr0 [h1 h2]]. inv h1.
+    - inv h2. move: H1 => [st0 [_ h1]]. inv h1. simpl. apply skips_delay.
+      by apply skips_nil. by simpl.
     - move: H => [tr1 [h1 h3]]. move: h1 => [st0 [[_ h1] h4]].
-      foo h4. foo h3. foo H0. foo h2. simpl in h0. absurd False.
-      done. have := cond_true h1 h0. by apply. 
-  - move => tr0 h0 [tr1 [h1 h2]]. move: h1 => [st0 [_ h3]]. foo h3. foo H1.
-    foo h2. simpl in h0. foo H2. apply skips_delay; last done. 
-    move: H1 => [tr0 [h1 h2]]. foo h1. 
-    - foo h2. move: H1 => [st0 [h1 h2]]. foo h2. apply skips_nil. 
-    - move: H => [tr1 [h1 h3]]. move: h1 => [st0 [h1 h4]]. foo h4. foo H2. 
-      foo h3. foo H0. foo H3. foo h2. simpl in h0. 
-      have h2: skips tr'1. apply IHn => {IHn}. have h2 := follows_hd H4. 
+      inv h4. inv h3. inv H0. inv h2. simpl in h0. absurd False.
+      done. have := cond_true h1 h0. by apply.
+  - move => tr0 h0 [tr1 [h1 h2]]. move: h1 => [st0 [_ h3]]. inv h3. inv H1.
+    inv h2. simpl in h0. inv H2. apply skips_delay; last done.
+    move: H1 => [tr0 [h1 h2]]. inv h1.
+    - inv h2. move: H1 => [st0 [h1 h2]]. inv h2. apply skips_nil.
+    - move: H => [tr1 [h1 h3]]. move: h1 => [st0 [h1 h4]]. inv h4. inv H2.
+      inv h3. inv H0. inv H3. inv h2. simpl in h0.
+      have h2: skips tr'1. apply IHn => {IHn}. have h2 := follows_hd H4.
       rewrite -h2 => {h2}. rewrite H0 => {H0}. rewrite /decr_y h0 => {h0}.
       rewrite /update. have ->: y =? y = true by apply Nat.eqb_refl.
-      by apply Sn_1. exists tr'0. split; first done. 
-      move: H1 => [st1 [_ h2]]. foo h2. simpl in H0. foo H2. foo H4.
-      apply follows_delay. foo H2. foo H5. apply follows_nil => //. 
-      exists tr'. split; first done. have h2 := follows_singleton H4. 
+      by apply Sn_1. exists tr'0. split; first done.
+      move: H1 => [st1 [_ h2]]. inv h2. simpl in H0. inv H2. inv H4.
+      apply follows_delay. inv H2. inv H5. apply follows_nil => //.
+      exists tr'. split; first done. have h2 := follows_singleton H4.
       have := follows_setoid_R (@singleton_setoid _) H4 (bisim_symmetric h2).
-      by apply. apply skips_delay. have h3 := follows_singleton H5. 
-      have := skips_setoid h2 h3. by apply. have h3 := follows_hd H5. 
+      by apply. apply skips_delay. have h3 := follows_singleton H5.
+      have := skips_setoid h2 h3. by apply. have h3 := follows_hd H5.
       rewrite -h3 => {h3}. clear h2 h0 H1 H5. have h0 := follows_hd H4 => {H4}.
-      rewrite -h0 => {h0}. rewrite H0 => {H0}. rewrite /update.    
+      rewrite -h0 => {h0}. rewrite H0 => {H0}. rewrite /update.
       rewrite yx. done.
-have h1 := semax_conseq_R h0 h2 => {h0 h2}. 
-have h0 := semax_assign ttS x incr_x. 
+have h1 := semax_conseq_R h0 h2 => {h0 h2}.
+have h0 := semax_assign ttS x incr_x.
 have h2 := semax_conseq_R (@Append_ttS _) h1 => {h1}.
 have h1 := semax_seq h2 h0 =>  {h2 h0}.
 have h0 := semax_conseq_R (@Append_ttS _) (semax_assign ttS y (fun st => st x)).
-have h2 := semax_seq h0 h1 => {h0 h1}.  
+have h2 := semax_seq h0 h1 => {h0 h1}.
 have h0 := semax_conseq_R (@Append_assoc_R _ _ _) h2 => {h2}.
 have h1: (Updt ttS y (fun st => st x) *** Skips) =>> Skips.
-* clear h0. move => tr0 [tr1 [h0 h1]]. simpl. move: h0 => [st0 [_ h0]]. 
-  foo h0. foo H1. foo h1. foo H2. apply skips_delay => //. rewrite H0.
-  rewrite /update. rewrite yx. done. 
+* clear h0. move => tr0 [tr1 [h0 h1]]. simpl. move: h0 => [st0 [_ h0]].
+  inv h0. inv H1. inv h1. inv H2. apply skips_delay => //. rewrite H0.
+  rewrite /update. rewrite yx. done.
 have h2 := semax_conseq_R (Append_monotone_L h1) h0 => {h0 h1}.
-have h0: x_is_zero ->> ttS; first done. 
+have h0: x_is_zero ->> ttS; first done.
 have h1: (ttS andS eval_true tt) ->> ttS; first done.
-have h3 := semax_conseq h1 (@Append_ttS _) h2 => {h2 h1}.  
-have h1 := semax_while h0 h3 => {h0 h3}.       
+have h3 := semax_conseq h1 (@Append_ttS _) h2 => {h2 h1}.
+have h1 := semax_while h0 h3 => {h0 h3}.
 have h0: (<<x_is_zero>> *** Iter ((Skips *** Updt ttS x incr_x)
-*** <<ttS>>) *** [| eval_false tt |]) =>> (Up 0). 
-* clear h1. move => tr0 h0. simpl. simpl in h0. 
+*** <<ttS>>) *** [| eval_false tt |]) =>> (Up 0).
+* clear h1. move => tr0 h0. simpl. simpl in h0.
   move: h0 => [tr1 [h0 h1]]. move: h0 => [st0 [h0 h2]]. rewrite /x_is_zero in h0.
-  foo h2. foo H1. foo h1. foo H2. move: H1 => [tr0 [h1 h2]].  
+  inv h2. inv H1. inv h1. inv H2. move: H1 => [tr0 [h1 h2]].
   have: forall n tr0 tr1, hd tr1 x = n ->
-   iter (append (append (fun tr => skips tr) (updt ttS x incr_x)) (dup ttS)) tr0 -> 
+   iter (append (append (fun tr => skips tr) (updt ttS x incr_x)) (dup ttS)) tr0 ->
    follows (singleton (eval_false tt)) tr0 tr1 -> up n (Tcons (hd tr1) tr1).
-  * clear tr' h0 tr0 h1 h2. cofix hcoind. move => n tr0 tr1 h0 h1 h2. foo h1. 
-    - foo h2. move: H1 => [st0 [h0 h1]]. rewrite /eval_false in h0. clear h1. 
-      rewrite tt_true in h0. foo h0. 
+  * clear tr' h0 tr0 h1 h2. cofix hcoind. move => n tr0 tr1 h0 h1 h2. inv h1.
+    - inv h2. move: H1 => [st0 [h0 h1]]. rewrite /eval_false in h0. clear h1.
+      rewrite tt_true in h0. inv h0.
     - move: H => [tr2 [h0 h1]]. move: h0 => [tr3 [h0 h3]].
-      have h4: forall tr3, skips tr3 -> 
+      have h4: forall tr3, skips tr3 ->
       forall tr2, follows (updt ttS x incr_x) tr3 tr2 ->
       forall tr, follows (dup ttS) tr2 tr ->
       forall tr0, follows (iter
           (append (append (fun tr : trace => skips tr)
            (updt ttS x incr_x)) (dup ttS))) tr tr0 ->
-      forall tr1, follows (singleton (eval_false tt)) tr0 tr1 ->   
+      forall tr1, follows (singleton (eval_false tt)) tr0 tr1 ->
       exists tr4 : trace, ((red_hd_x (Tcons (hd tr1) tr1) (Tcons (hd tr4) tr4)) /\
         (hd tr4 x = S (hd tr1 x)) /\
         (iter (append
          (append (fun tr : trace => skips tr)
          (updt ttS x incr_x)) (dup ttS)) tr4) /\
          (follows (singleton (eval_false tt)) tr4 tr4)).
-       * clear hcoind tr0 tr1 h2 tr H0 tr2 h1 tr3 h0 h3. induction 1. 
-          - move => tr0 h0 tr1 h1 tr2 h2 tr3 h3. foo h0. 
-            move: H1 => [st0 [h0 h4]]. foo h4. foo h1. foo H1. clear h0. 
-            foo H3. foo h2. move: H1 => [st1 [h0 h1]]. foo h1. foo H2. 
-            simpl in H0. foo H4. clear h0. foo H3. foo h3. foo H4. exists tr'.
-            have h0 := follows_hd H5. 
-            have h1 := follows_singleton H5. 
+       * clear hcoind tr0 tr1 h2 tr H0 tr2 h1 tr3 h0 h3. induction 1.
+          - move => tr0 h0 tr1 h1 tr2 h2 tr3 h3. inv h0.
+            move: H1 => [st0 [h0 h4]]. inv h4. inv h1. inv H1. clear h0.
+            inv H3. inv h2. move: H1 => [st1 [h0 h1]]. inv h1. inv H2.
+            simpl in H0. inv H4. clear h0. inv H3. inv h3. inv H4. exists tr'.
+            have h0 := follows_hd H5.
+            have h1 := follows_singleton H5.
             split. apply red_hd_x_tau. by simpl.
             apply red_hd_x_stop.
-            simpl. rewrite /update. 
+            simpl. rewrite /update.
             have ->: x =? x = true by apply Nat.eqb_refl.
             rewrite /incr_x.
             have ->: st0 x + 1 = S (st0 x) by lia. by auto with arith. rewrite H0.
@@ -218,29 +214,30 @@ have h0: (<<x_is_zero>> *** Iter ((Skips *** Updt ttS x incr_x)
             simpl. rewrite H0. rewrite /update. have h: x =? x = true by apply Nat.eqb_refl.
             rewrite h => {h}.  split. by apply Sn. split.
             by apply H1. have := follows_setoid _ H5 _ (bisim_symmetric h1). apply.
-            move => tr0 h2 tr1 h3. move: h2 => [st1 [h2 h4]]. foo h4.
-            exists st1. split => //. have := bisim_symmetric h3. by apply. 
-            by apply bisim_reflexive. 
-          - move => tr0 h0 tr1 h1 tr2 h2 tr3 h3. foo h0. 
-            have h0 := IHskips _ H4 => {IHskips}. foo h1. 
-            have h1 := h0 _ H5 => {h0}. foo h2. 
-            have h2 := h1 _ H6 => {h1}. foo h3. 
+            move => tr0 h2 tr1 h3. move: h2 => [st1 [h2 h4]]. inv h4.
+            exists st1. split => //. have := bisim_symmetric h3. by apply.
+            by apply bisim_reflexive.
+          - move => tr0 h0 tr1 h1 tr2 h2 tr3 h3. inv h0.
+            have h0 := IHskips _ H4 => {IHskips}. inv h1.
+            have h1 := h0 _ H5 => {h0}. inv h2.
+            have h2 := h1 _ H6 => {h1}. inv h3.
             have h3 := h2 _ H7 => {h2}. move: h3 => [tr0 [h3 [h0 [h1 h2]]]].
-            simpl. rewrite -H0.  
+            simpl. rewrite -H0.
             have h4 := follows_hd H4; rewrite h4 => {H4}.
             have h5 := follows_hd H5; rewrite h5  => {H5}.
-            have h6 := follows_hd H6; rewrite h6  => {H6}. 
-            have h7 := follows_hd H7; rewrite h7 => {H7}. 
-            rewrite -h0. 
-            exists tr0. split => //. clear h1 h2. 
-            apply red_hd_x_tau. simpl. reflexivity. foo h3. 
-            absurd False. done. apply H3. reflexivity. apply red_hd_x_tau. 
-            rewrite -H0; rewrite h4. rewrite h5; rewrite h6; rewrite h7. 
-            reflexivity. by apply H5.
-     have h := h4 _ h0 _ h3 _ h1 _ H0 _ h2 => {h4 h0 h3 h1 H0 h2}. 
+            have h6 := follows_hd H6; rewrite h6  => {H6}.
+            have h7 := follows_hd H7; rewrite h7 => {H7}.
+            rewrite -h0.
+            exists tr0. split => //. clear h1 h2.
+            apply red_hd_x_tau; first by simpl; reflexivity.
+            inv h3; first by absurd False=>//; apply: H3; reflexivity.
+            apply red_hd_x_tau.
+            by rewrite -H0 h4 h5 h6 h7.
+          by apply H5.
+     have h := h4 _ h0 _ h3 _ h1 _ H0 _ h2 => {h4 h0 h3 h1 H0 h2}.
      move: h => [tr4 [h4 [h7 [h5 h6]]]].
-     have := up_intro _ h4. apply. reflexivity. 
-     have := hcoind _ _ _ _ _ h6. apply. by apply h7. apply h5. 
-     move => h3. have := h3 _ _ _ h0 h1 h2. by apply. 
-  have := semax_conseq_R h0 h1. by apply. 
+     apply: (up_intro _ h4)=>//.
+     apply: (hcoind _ _ _ _ _ h6). by apply h7. apply h5.
+     move => h3. by apply: (h3 _ _ _ h0 h1 h2).
+  by apply: (semax_conseq_R h0 h1).
 Qed.
